add eq and uni

combinator.v
@@ -1,5 +1,4 @@
-Require Import FunctionalExtensionality ProofIrrelevance ClassicalDescription.
-Require Import ClassicalChoice ChoiceFacts.
+Require Import FunctionalExtensionality ClassicalDescription.
 Require Import Coq.Logic.Eqdep_dec.
 Require Import Program.
 Set Implicit Arguments.
@@ -7,53 +6,68 @@ Set Automatic Coercions Import.
 Require Import ssp.
 
 Arguments proj1_sig {A P} e.
+Arguments projT1 {A P} x.
 
 Section Constant_SSPF.
 
 Variable A : Type.
 
-Definition const_Fn :=
-  (PFunctor.mk_data (fun X => A) (fun X Y (f: X -> Y) x => x) (fun _ _ _ => False)).
+Definition const_eq (X : Type) (EQ: X -> X -> Prop) : A -> A -> Prop := (@eq A).
+
+Program Definition const_Fn :=
+  (@PFunctor.mk_data (fun X => A) (fun _ _ _ => False) const_eq
+                     (fun X Y (f: X -> Y) x => x) (fun _ _ a _ => a) _).
 
 Definition const_embed X (a: A) (s: unit) : X + A := inr a.
 
 Program Definition Const : SSPF.t := 
-  @SSPF.mk const_Fn unit A 
-          (PNatTrans.mk _ _ const_embed _ _) _ _.
+  @SSPF.mk const_Fn unit A const_embed _ _ _ _ _.
 Next Obligation.
-  unfold const_embed. split; intros.
-  - inversion H.
-  - inversion H. inversion EQ.
-Qed.
+  inversion H.
+Defined.
 Next Obligation.
-  exists m. eauto.
-Qed.
+  unfold const_embed in X0.
+  inversion X0. inversion EQ.
+Defined.
+Next Obligation.
+  split; unfold SPUF.u_eq, const_eq, const_embed; intros.
+  - split; intros.
+    + subst. tauto.
+    + inversion H0.
+  - destruct H. specialize (H tt fx1).
+    destruct H. specialize (H eq_refl).
+    inversion H. auto.
+Defined.
 Next Obligation.
   unfold const_embed in EQ.
   apply equal_f with tt in EQ.
   inversion EQ. auto.
-Qed.
+Defined.
 
-(* @jeehoonkang: consider Empty_set.. *)
 End Constant_SSPF.
 
 Section Identity_SSPF.
 
-Definition ident_embed X (x: X) (s: unit) : X + unit := inl x.
+Definition ident_embed X (x: X) (s: unit) : X + False := inl x.
 
 Program Definition Ident : SSPF.t := 
-  @SSPF.mk PFunctor.id_data unit unit
-          (PNatTrans.mk _ _ ident_embed _ _) _ _.
+  @SSPF.mk ident_Fn unit False ident_embed _ _ _ _ _.
 Next Obligation.
-  unfold ident_embed. split; intros.
+  unfold ident_embed.
+  apply (SPUF._u_mem _ tt). auto.
+Defined.
+Next Obligation.
+  unfold ident_embed in X0.
+  inversion X0. inversion EQ. constructor.
+Defined.
+Next Obligation.
+  split; unfold ident_embed, SPUF.u_eq; intros.
+  - split; intros.
+    + destruct e.
+    + inversion H0. inversion H1. subst. auto.
   - destruct H.
-    apply (SPUF._u_rel _ tt). auto.
-  - inversion H. inversion EQ.
-    constructor.
-Qed.  
-Next Obligation.
-  exfalso. specialize (CONST m m). eauto.
-Qed.
+    specialize (H0 tt fx1 fx2). tauto.
+Defined.
 Next Obligation.
   apply equal_f with tt in EQ.
   inversion EQ. auto.
@@ -71,14 +85,34 @@ Definition coprod_map X Y (f: X -> Y) x :=
   | inr xr => inr (G.(PFunctor.map) f xr)
   end.
 
-Inductive coprod_rel X : X -> (F X + G X) -> Prop :=
-| _coprod_rell x fx (RF: F.(PFunctor.rel) x fx) : coprod_rel x (inl fx)
-| _coprod_relr x gx (RG: G.(PFunctor.rel) x gx) : coprod_rel x (inr gx).
+Definition coprod_mem X (x: F X + G X) : X -> Type :=
+  match x with
+  | inl fx => F.(PFunctor.mem) fx
+  | inr gx => G.(PFunctor.mem) gx end.
 
-Definition coprod_Fn :=
-  (PFunctor.mk_data (fun X => sum (F X) (G X)) coprod_map coprod_rel).
+Inductive coprod_eq X (EQ: X -> X -> Prop) : (F X + G X) -> (F X + G X) -> Prop :=
+  | _copr_eql fx1 fx2 : F.(PFunctor.eq) EQ fx1 fx2 -> coprod_eq EQ (inl fx1) (inl fx2)
+  | _copr_eqr gx1 gx2 : G.(PFunctor.eq) EQ gx1 gx2 -> coprod_eq EQ (inr gx1) (inr gx2).
 
-(* @jeehoonkang: consider `match x, s with | inl x', inl (inl _) => ... *)
+Definition coprod_uni X Y (x: F X + G X) (ALL: forall y, coprod_mem x y -> Y)
+  : F Y + G Y.
+  destruct x.
+  - apply (inl (F.(PFunctor.uni) f (fun y r => ALL _ r))).
+  - apply (inr (G.(PFunctor.uni) f (fun y r => ALL _ r))).
+Defined.
+
+Program Definition coprod_Fn :=
+  (@PFunctor.mk_data (fun X => sum (F X) (G X)) coprod_mem coprod_eq
+                     coprod_map coprod_uni _).
+Next Obligation.
+Proof.
+  unfold coprod_map. destruct a; unfold coprod_uni; f_equal.
+  - apply F.(PFunctor.uni_correct).
+    intros. apply INV.
+  - apply G.(PFunctor.uni_correct).
+    intros. apply INV.
+Defined.
+
 Definition coprod_embed X (x: sum (F X) (G X))
            (s: sum (sum unit F.(SSPF.Sh)) (sum unit G.(SSPF.Sh))) :=
   match x with
@@ -105,56 +139,79 @@ Definition coprod_embed X (x: sum (F X) (G X))
   end.
 
 Program Definition Coprod : SSPF.t := 
-  @SSPF.mk coprod_Fn _ _
-          (PNatTrans.mk _ _ coprod_embed _ _) _ _.
+  @SSPF.mk coprod_Fn _ _ coprod_embed _ _ _ _ _.
 Next Obligation.
-  extensionality s. unfold coprod_embed, coprod_map.
+  unfold coprod_embed. destruct fx;
+  apply SSPF.mem_nat1 in X0; destruct X0.
+  - apply (SPUF._u_mem _ (inl (inr s))). rewrite EQ. auto.
+  - apply (SPUF._u_mem _ (inr (inr s))). rewrite EQ. auto.
+Defined.
+Next Obligation.
+Proof.
+  destruct fx;
+  inversion X0; subst; destruct s;
+  try destruct s; inversion EQ; apply SSPF.mem_nat2.
+  - apply (SPUF._u_mem _ s).
+    destruct ((SSPF.emb F) X f); inversion H0. auto.
+  - apply (SPUF._u_mem _ s).
+    destruct ((SSPF.emb G) X f); inversion H0. auto.
+Defined.
+Next Obligation.
+Proof.
+  unfold coprod_embed, coprod_map.
   destruct x; destruct s; destruct s; try eauto;
-  rewrite PNatTrans.map_nat; simpl; unfold SPUF.map;
+  rewrite SSPF.map_nat; simpl; unfold SPUF.map;
   [destruct ((SSPF.emb F) X f0) | destruct ((SSPF.emb G) X f0)]; eauto.
-Qed.
+Defined.
 Next Obligation.
-  unfold coprod_embed. split; intros.
-  - destruct H.
-    + rewrite (PNatTrans.rel_nat F.(SSPF.emb)) in RF.
-      destruct RF.
-      apply (SPUF._u_rel _ (inl (inr s))).
-      destruct (u s); inversion EQ. auto.
-    + rewrite (PNatTrans.rel_nat G.(SSPF.emb)) in RG.
-      destruct RG.
-      apply (SPUF._u_rel _ (inr (inr s))).
-      destruct (u s); inversion EQ. auto.
-  - destruct fx; constructor;
-    inversion H; subst; destruct s; try destruct s; inversion EQ.
-    + apply (PNatTrans.rel_nat F.(SSPF.emb)).
-      apply (SPUF._u_rel _ s).
-      destruct ((SSPF.emb F) X f); inversion EQ. auto.
-    + apply (PNatTrans.rel_nat G.(SSPF.emb)).
-      apply (SPUF._u_rel _ s).
-      destruct ((SSPF.emb G) X f); inversion EQ. auto.
-Qed.
-Next Obligation.
-  unfold coprod_embed in CONST.
-  destruct m.
-  - assert (H : forall (s : SSPF.Sh F) (x : ()), (SSPF.emb F) unit f s <> inl x).
-    { intros.
-      specialize (CONST (inl (inr s)) tt). simpl in CONST.
-      destruct ((SSPF.emb F) unit f).
-      - destruct u; exfalso; auto. 
-      - intro. inversion H.
-    }
-    apply SSPF.uni in H; destruct H; unfold coprod_map.
-    exists (inl x); f_equal; apply H.
-  - assert (H : forall (s : SSPF.Sh G) (x : ()), (SSPF.emb G) unit f s <> inl x).
-    { intros.
-      specialize (CONST (inr (inr s)) tt). simpl in CONST.
-      destruct ((SSPF.emb G) unit f).
-      - destruct u; exfalso; auto.
-      - intro. inversion H.
-    }
-    apply SSPF.uni in H; destruct H; unfold coprod_map.
-    exists (inr x); f_equal; apply H.
-Qed.
+  destruct fx1, fx2; split; intros; inversion H; subst.
+  - unfold SPUF.u_eq, coprod_embed; apply SSPF.eq_nat in H2; split; intros.
+    + destruct s; destruct s; split; intro; auto;
+      destruct (SSPF.emb F X f) eqn : EQ1; destruct (SSPF.emb F X f0) eqn : EQ2;
+      inversion H0; destruct H2;
+      try apply H1 in EQ1; try rewrite EQ1 in EQ2; inversion EQ2; auto.
+      apply H1 in EQ2. rewrite EQ1 in EQ2. inversion EQ2.
+    + destruct s; destruct s; inversion H0; inversion H1. inversion H2.
+      destruct (SSPF.emb F X f) eqn : EQ1; destruct (SSPF.emb F X f0) eqn : EQ2;
+      inversion H0; inversion H1; subst.
+      apply (H6 _ _ _ EQ1 EQ2).
+  - constructor. apply SSPF.eq_nat. constructor.
+    + intros. split; intros;
+      specialize (H0 (inl (inr s)) (inr (inl e))); unfold coprod_embed in H0;
+      rewrite H2 in H0; destruct H0.
+      * specialize (H0 eq_refl).
+        destruct (SSPF.emb F X f0); inversion H0. auto.
+      * specialize (H3 eq_refl).
+        destruct (SSPF.emb F X f); inversion H3. auto.
+    + intros. specialize (H1 (inl (inr s)) x1 x2); simpl in H1.
+      rewrite H2 in H1. rewrite H3 in H1.
+      apply (H1 eq_refl eq_refl).
+  - specialize (H0 (inl (inl tt)) (inl true)). unfold coprod_embed in H0.
+    destruct H0. specialize (H0 eq_refl). inversion H0.
+  - specialize (H0 (inl (inl tt)) (inl true)). unfold coprod_embed in H0.
+    destruct H0. specialize (H2 eq_refl). inversion H2.
+ - unfold SPUF.u_eq, coprod_embed; apply SSPF.eq_nat in H2; split; intros.
+    + destruct s; destruct s; split; intro; auto;
+      destruct (SSPF.emb G X f) eqn : EQ1; destruct (SSPF.emb G X f0) eqn : EQ2;
+      inversion H0; destruct H2;
+      try apply H1 in EQ1; try rewrite EQ1 in EQ2; inversion EQ2; auto.
+      apply H1 in EQ2. rewrite EQ1 in EQ2. inversion EQ2.
+    + destruct s; destruct s; inversion H0; inversion H1. inversion H2.
+      destruct (SSPF.emb G X f) eqn : EQ1; destruct (SSPF.emb G X f0) eqn : EQ2;
+      inversion H0; inversion H1; subst.
+      apply (H6 _ _ _ EQ1 EQ2).
+  - constructor. apply SSPF.eq_nat. constructor.
+    + intros. split; intros;
+      specialize (H0 (inr (inr s)) (inr (inr e))); unfold coprod_embed in H0;
+      rewrite H2 in H0; destruct H0.
+      * specialize (H0 eq_refl).
+        destruct (SSPF.emb G X f0); inversion H0. auto.
+      * specialize (H3 eq_refl).
+        destruct (SSPF.emb G X f); inversion H3. auto.
+    + intros. specialize (H1 (inr (inr s)) x1 x2); simpl in H1.
+      rewrite H2 in H1. rewrite H3 in H1.
+      apply (H1 eq_refl eq_refl).
+Defined.
 Next Obligation.
 Proof.
   destruct m; destruct n; unfold coprod_embed in EQ.
@@ -176,7 +233,6 @@ Qed.
 
 End Coproduct_SSPF.
 
-
 Section Product_SSPF.
 
 Variable F G: SSPF.t.
@@ -186,12 +242,32 @@ Definition prod_map X Y (f: X -> Y) x :=
   | (xl, xr) => (F.(PFunctor.map) f xl, G.(PFunctor.map) f xr)
   end.
 
-Inductive prod_rel X : X -> (prod (F X) (G X)) -> Prop :=
-| _prod_rell x fx gx (RF: F.(PFunctor.rel) x fx) : prod_rel x (fx, gx)
-| _prod_relr x fx gx (RG: G.(PFunctor.rel) x gx) : prod_rel x (fx, gx).
+Definition prod_mem X (a: prod (F X) (G X)) (x: X) : Type :=
+  match a with
+  | (fx, gx) => (F.(PFunctor.mem) fx x) + (G.(PFunctor.mem) gx x) end.
 
-Definition prod_Fn :=
-  (PFunctor.mk_data (fun X => prod (F X) (G X)) prod_map prod_rel).
+Definition prod_eq X (EQ: X -> X -> Prop) (x1 x2: F X * G X) : Prop :=
+  match x1, x2 with
+  | (fx1, gx1), (fx2, gx2) => F.(PFunctor.eq) EQ fx1 fx2 /\ G.(PFunctor.eq) EQ gx1 gx2
+  end.
+
+Definition prod_uni X Y (x: F X * G X) (ALL: forall y, prod_mem x y -> Y) 
+  : F Y * G Y.
+  destruct x.
+  apply (F.(PFunctor.uni) f (fun y r => ALL _ (inl r)),
+         G.(PFunctor.uni) f0 (fun y r => ALL _ (inr r))).
+Defined.
+
+Program Definition prod_Fn :=
+  (@PFunctor.mk_data (fun X => prod (F X) (G X)) prod_mem prod_eq prod_map prod_uni _).
+Next Obligation.
+Proof.
+  unfold prod_map. unfold prod_uni. f_equal.
+  - apply F.(PFunctor.uni_correct).
+    intros. apply INV.
+  - apply G.(PFunctor.uni_correct).
+    intros. apply INV.
+Defined.
 
 Definition prod_embed X (x: prod (F X) (G X)) (s: sum F.(SSPF.Sh) G.(SSPF.Sh)) :=
   match x with
@@ -211,54 +287,71 @@ Definition prod_embed X (x: prod (F X) (G X)) (s: sum F.(SSPF.Sh) G.(SSPF.Sh)) :
   end.
 
 Program Definition Prod : SSPF.t := 
-  @SSPF.mk prod_Fn (sum F.(SSPF.Sh) G.(SSPF.Sh)) (sum F.(SSPF.Ext) G.(SSPF.Ext))
-          (PNatTrans.mk _ _ prod_embed _ _) _ _.
+  @SSPF.mk prod_Fn _ _ prod_embed _ _ _ _ _.
+Next Obligation.
+  unfold prod_embed. inversion X0;
+  apply SSPF.mem_nat1 in X1; inversion X1; subst.
+  - apply (SPUF._u_mem _ (inl s)).
+    rewrite EQ. auto.
+  - apply (SPUF._u_mem _ (inr s)).
+    rewrite EQ. auto.
+Defined.
+Next Obligation.
+  unfold prod_embed in X0. inversion X0. subst.
+  destruct s.
+  - apply inl.
+    apply F.(SSPF.mem_nat2).
+    apply (SPUF._u_mem _ s).
+    destruct ((SSPF.emb F) X f); inversion EQ. auto.
+  - apply inr.
+    apply G.(SSPF.mem_nat2).
+    apply (SPUF._u_mem _ s).
+    destruct ((SSPF.emb G) X f0); inversion EQ. auto.
+Defined.
 Next Obligation.  
-  extensionality s. unfold prod_map, prod_embed. repeat rewrite PNatTrans.map_nat.
-  destruct s; simpl; unfold SPUF.map;
-  [destruct ((SSPF.emb F) X f0) | destruct ((SSPF.emb G) X f1)]; eauto.
-Qed.
+  unfold prod_map, prod_embed.
+  destruct s; rewrite SSPF.map_nat; unfold SPUF.map.
+  - destruct (SSPF.emb F X f0 s); auto.
+  - destruct (SSPF.emb G X f1 s); auto.
+Defined.
 Next Obligation.
-  unfold prod_embed. split; intros.
-  - inversion H; subst.
-    + apply (PNatTrans.rel_nat F.(SSPF.emb)) in RF.
-      inversion RF.
-      subst.
-      (* Set Printing All. idtac. *)
-      apply (SPUF._u_rel _ (inl s)).
-      rewrite EQ. auto.
-    + apply (PNatTrans.rel_nat G.(SSPF.emb)) in RG.
-      inversion RG.
-      subst.      
-      apply (SPUF._u_rel _ (inr s)).
-      rewrite EQ. auto.
-  - inversion H. subst.
-    destruct s.
-    + apply _prod_rell.
-      apply (PNatTrans.rel_nat F.(SSPF.emb)).
-      apply (SPUF._u_rel _ s).
-      destruct ((SSPF.emb F) X f); inversion EQ. auto.
-    + apply _prod_relr.
-      apply (PNatTrans.rel_nat G.(SSPF.emb)).
-      apply (SPUF._u_rel _ s).
-      destruct ((SSPF.emb G) X f0); inversion EQ. auto.
-Qed.
-Next Obligation.
-  unfold prod_embed in CONST.
-  assert (H1 : forall s x, (SSPF.emb F) unit f s <> inl x).
-  { intros.
-    specialize (CONST (inl s) tt). simpl in CONST.
-    destruct ((SSPF.emb F) unit f);
-    [exfalso; destruct u; eauto | intro; inversion H].
-  }
-  assert (H2 : forall s x, (SSPF.emb G) unit f0 s <> inl x). intros.
-  { specialize (CONST (inr s) tt). simpl in CONST.
-    destruct ((SSPF.emb G) unit f0);
-    [exfalso; destruct u; eauto | intro; inversion H].
-  }
-  apply SSPF.uni in H1. apply SSPF.uni in H2. destruct H1, H2.
-  exists (x, x0).
-  unfold prod_map. rewrite H. rewrite H0. eauto.
+Proof.
+  split; unfold SPUF.u_eq, prod_embed, prod_eq; intros.
+  - destruct H. apply SSPF.eq_nat in H. apply SSPF.eq_nat in H0.
+    destruct H, H0. split; intros.
+    + split; intros.
+      destruct s;
+      [destruct (SSPF.emb F X f) eqn : EQ1; destruct (SSPF.emb F X f1) eqn : EQ2;
+       inversion H3; apply H in EQ2; rewrite EQ2 in EQ1; inversion EQ1; auto |
+       destruct (SSPF.emb G X f0) eqn : EQ1; destruct (SSPF.emb G X f2) eqn : EQ2;
+       inversion H3; apply H0 in EQ2; rewrite EQ2 in EQ1; inversion EQ1; auto ].
+      destruct s;
+      [destruct (SSPF.emb F X f) eqn : EQ1; destruct (SSPF.emb F X f1) eqn : EQ2;
+       inversion H3; apply H in EQ1; rewrite EQ1 in EQ2; inversion EQ2; auto |
+       destruct (SSPF.emb G X f0) eqn : EQ1; destruct (SSPF.emb G X f2) eqn : EQ2;
+       inversion H3; apply H0 in EQ1; rewrite EQ1 in EQ2; inversion EQ2; auto ].
+    + destruct s.
+      destruct (SSPF.emb F X f1)  eqn : EQ1; destruct (SSPF.emb F X f)  eqn : EQ2;
+      inversion H3; inversion H4; subst.
+      apply (H1 _ _ _ EQ1 EQ2).
+      destruct (SSPF.emb G X f2)  eqn : EQ1; destruct (SSPF.emb G X f0)  eqn : EQ2;
+      inversion H3; inversion H4; subst.
+      apply (H2 _ _ _ EQ1 EQ2).
+  - split; apply SSPF.eq_nat; destruct H; split; intros.
+    + split; intros; specialize (H (inl s) (inl e)); simpl in H; rewrite H1 in H.
+      * destruct H. specialize (H eq_refl).
+        destruct (SSPF.emb F X f); inversion H; auto.
+      * destruct H. specialize (H2 eq_refl).
+        destruct (SSPF.emb F X f1); inversion H2; auto.
+    + specialize (H0 (inl s)); simpl in H0; rewrite H1 in H0; rewrite H2 in H0.
+      apply H0; auto.
+    + split; intros; specialize (H (inr s) (inr e)); simpl in H; rewrite H1 in H.
+      * destruct H. specialize (H eq_refl).
+        destruct (SSPF.emb G X f0); inversion H; auto.
+      * destruct H. specialize (H2 eq_refl).
+        destruct (SSPF.emb G X f2); inversion H2; auto.
+    + specialize (H0 (inr s)); simpl in H0; rewrite H1 in H0; rewrite H2 in H0.
+      apply H0; auto.
 Qed.
 Next Obligation.
   f_equal; apply SSPF.inj; extensionality s.
@@ -280,48 +373,404 @@ Variable A : Type.
 Definition exp_map X Y (f: X -> Y) (x: A -> X) :=
   fun (a: A) => f (x a).
 
-Inductive exp_rel X : X -> (A -> X) -> Prop :=
-| _exp_rel f a : exp_rel (f a) f.
+Inductive on_image X : (A -> X) -> X -> Type :=
+  | _on_image f a : on_image f (f a).
 
-Definition exp_Fn := (PFunctor.mk_data (fun X => A -> X) exp_map exp_rel).
+Definition exp_uni X Y (x: A -> X) (ALL: forall y, on_image x y -> Y)
+  : A -> Y := fun y => (ALL _ (_on_image x y)).
+
+Definition exp_eq X (EQ: X -> X -> Prop) (x1 x2: A -> X) : Prop :=
+  forall a, EQ (x1 a) (x2 a).
+
+Program Definition exp_Fn :=
+  (@PFunctor.mk_data (fun X => A -> X) on_image exp_eq exp_map exp_uni _).
+Next Obligation.
+Proof.
+  unfold exp_map. unfold exp_uni.
+  extensionality s.
+  rewrite INV. auto.
+Defined.
 
 Definition exp_embed X (x: A -> X) (s: A) : (X + False) := inl (x s).
 
 Program Definition Expn : SSPF.t := 
-  @SSPF.mk exp_Fn _ _
-          (PNatTrans.mk _ _ exp_embed _ _) _ _.
+  @SSPF.mk exp_Fn _ _ exp_embed _ _ _ _ _.
 Next Obligation.
-  unfold exp_embed. split; intros.
+  unfold exp_embed. destruct X0.
+  apply (SPUF._u_mem _ a). auto.
+Defined.
+Next Obligation.
+  unfold exp_embed. inversion X0.
+  subst. inversion EQ. constructor.
+Defined.
+Next Obligation.
+  unfold exp_embed, exp_eq. split; intros.
+  - unfold SPUF.u_eq; split; intros.
+    + destruct e.
+    + inversion H0; inversion H1. apply H.
   - destruct H.
-    apply (SPUF._u_rel _ a). auto.
-  - inversion H. subst. inversion EQ.
-    constructor.
-Qed.
-Next Obligation.
-  unfold exp_embed, exp_map in *.
-  exists (fun (a: A) => (CONST a (m a)) eq_refl).
-  extensionality s. destruct (m s). auto.
-Qed.
+    apply (H0 a); auto.
+Defined.
 Next Obligation.
   unfold exp_embed in EQ.
   extensionality s. apply equal_f with s in EQ.
   inversion EQ. auto.
-Qed.
+Defined.
 
 End Exponential_SSPF.
+
+Section Dependent_function_SSPF.
+
+Variable A: Type.
+Variable B: A -> SSPF.t.
+
+Definition depfun_map X Y (f: X -> Y) (x: forall a : A, B a X) :=
+  fun (a: A) => (B a).(PFunctor.map) f (x a).
+
+Definition depfun_mem X (f: forall a : A, B a X) (x: X) : Type :=
+  sigT (fun a => (B a).(PFunctor.mem) (f a) x).
+
+Definition depfun_eq X (EQ: X -> X -> Prop) (x1 x2: forall a : A, B a X) : Prop :=
+  forall a, (B a).(PFunctor.eq) EQ (x1 a) (x2 a).
+
+Definition depfun_uni X Y (x: forall a : A, B a X)
+           (ALL: forall y, depfun_mem x y -> Y) : forall a : A, B a Y :=
+  (fun a => (B a).(PFunctor.uni) (x a)
+      (fun y r =>ALL y (existT (fun a => (B a).(PFunctor.mem) (x a) y) _ r))).
+
+Program Definition depfun_Fn :=
+  (@PFunctor.mk_data (fun X => forall a : A, B a X)
+                     depfun_mem depfun_eq depfun_map depfun_uni _).
+Next Obligation.
+Proof.
+  unfold depfun_map. unfold depfun_uni.
+  extensionality s.
+  apply (B s).(PFunctor.uni_correct).
+  intros. apply INV.
+Defined.
+
+Definition depfun_embed X (x: forall a : A, B a X) (s: sigT (fun a => SSPF.Sh (B a)))
+: (X + (sigT (fun a => SSPF.Ext (B a)))) :=
+  match s with
+  | existT _ a sh =>
+    match (B a).(SSPF.emb) _ (x a) sh with
+    | inl v => inl v
+    | inr v => inr (existT _ a v)
+    end
+  end.
+
+Program Definition Depend_Fun : SSPF.t := 
+  @SSPF.mk depfun_Fn _ _ depfun_embed _ _ _ _ _.
+Next Obligation.
+  unfold depfun_embed. inversion X0.
+  apply (B x0).(SSPF.mem_nat1) in X1.
+  inversion X1. subst.
+  apply (SPUF._u_mem _ (existT _ x0 s)).
+  rewrite EQ. auto.
+Defined.
+Next Obligation.
+  inversion X0. subst.
+  destruct s.
+  apply (existT _ x0).
+  apply (B x0).(SSPF.mem_nat2).
+  apply (SPUF._u_mem _ s). simpl in *.
+  destruct ((SSPF.emb (B x0)) X (fx x0)); inversion EQ. auto.
+Defined.
+Next Obligation.
+  unfold depfun_map. unfold depfun_embed.
+  rewrite SSPF.map_nat. unfold SPUF.map.
+  destruct ((SSPF.emb (B s)) X (x s)); auto.
+Defined.
+Next Obligation.
+  unfold depfun_eq, depfun_embed; split; intros.
+  - split; intros; destruct s; specialize (H x); apply SSPF.eq_nat in H; destruct H.
+    + split; intros.
+      destruct (SSPF.emb (B x) X (fx1 x)) eqn : EQ1; inversion H1.
+      apply H in EQ1. rewrite EQ1. auto.
+      destruct (SSPF.emb (B x) X (fx2 x)) eqn : EQ1; inversion H1.
+      apply H in EQ1. rewrite EQ1. auto.
+    + destruct (SSPF.emb (B x) X (fx1 x)) eqn : EQ1; inversion H0;
+      destruct (SSPF.emb (B x) X (fx2 x)) eqn : EQ2; inversion H1; subst.
+      apply (H2 _ _ _ EQ1 EQ2).
+  - destruct H. apply SSPF.eq_nat. split; intros.
+    + split; intros;
+      specialize (H (existT _ a s) (existT _ a e)); simpl in H; destruct H.
+      * rewrite H1 in H. specialize (H eq_refl). 
+        destruct (SSPF.emb (B a) X (fx2 a)); inversion H.
+        dependent destruction H4. auto.
+      * rewrite H1 in H2. specialize (H2 eq_refl). 
+        destruct (SSPF.emb (B a) X (fx1 a)); inversion H2.
+        dependent destruction H4. auto.
+    + specialize (H0 (existT _ a s) x1 x2). simpl in H0.
+      rewrite H1 in H0; rewrite H2 in H0.
+      apply H0; auto.
+Defined.
+Next Obligation.
+  extensionality s. apply SSPF.inj.
+  extensionality sh.
+  unfold depfun_embed in EQ.
+  apply equal_f with (existT _ s sh) in EQ.
+  destruct ((SSPF.emb (B s)) X (m s)), ((SSPF.emb (B s)) X (n s));
+  inversion EQ; auto.
+  dependent destruction H0.
+  auto.
+Qed.
+
+End Dependent_function_SSPF.
+
+Section Dependent_sum_SSPF.
+
+Variable A: Type.
+Variable B: A -> SSPF.t.
+
+Definition depsum_map X Y (f: X -> Y) (x: sigT (fun a => (B a) X)) : (sigT (fun a => (B a) Y)) :=
+  match x with
+  | existT _ a x' => existT _ a ((B a).(PFunctor.map) f x') end.
+
+Definition depsum_mem X (x: sigT (fun a => (B a) X)) : X -> Type :=
+  match x with
+  | existT _ a x' => (B a).(PFunctor.mem) x' end.
+
+Inductive depsum_eq X (EQ: X -> X -> Prop)
+  : (sigT (fun a => (B a) X)) -> (sigT (fun a => (B a) X)) -> Prop :=
+  | _depsum_eq a fx1 fx2 : (B a).(PFunctor.eq) EQ fx1 fx2 ->
+                           depsum_eq EQ (existT _ a fx1) (existT _ a fx2).
+
+Definition depsum_uni X Y (x: sigT (fun a => (B a) X))
+           (ALL: forall y, depsum_mem x y -> Y) : (sigT (fun a => (B a) Y)).
+  destruct x.
+  apply (existT _ x ((B x).(PFunctor.uni) f (fun x0 r => ALL _ r))).
+Defined.
+
+Program Definition depsum_Fn :=
+  (@PFunctor.mk_data (fun X => sigT (fun a => (B a) X)) depsum_mem depsum_eq
+                     depsum_map depsum_uni _).
+Next Obligation.
+Proof.
+  unfold depsum_map. unfold depsum_uni.
+  f_equal. apply (B a).(PFunctor.uni_correct).
+  intros. apply INV.
+Defined.
+
+Definition depsum_embed X (x: sigT (fun a => (B a) X))
+           (s: sigT (fun a => sum unit (B a).(SSPF.Sh))) :
+  sum X (sum bool (sigT (fun a => (B a).(SSPF.Ext)))) :=
+match x with
+| existT _ a x' =>
+  match s with
+  | existT _ a' sh =>
+    match (excluded_middle_informative (a = a')) with
+    | left pf =>
+      match sh with
+      | inl _ => inr (inl true)
+      | inr sh' =>
+        match (B a').(SSPF.emb) _ (eq_rect _ (fun y => (B y) X) x' _ pf) sh' with
+        | inl a => inl a
+        | inr b => inr (inr (existT _ a' b)) end
+      end
+    | right _ => inr (inl false)
+    end
+  end
+end.
+
+Program Definition Depend_Sum : SSPF.t :=
+  @SSPF.mk depsum_Fn _ _ depsum_embed _ _ _ _ _.
+Next Obligation.
+  unfold depsum_embed. simpl in X0.
+  apply (B fx).(SSPF.mem_nat1) in X0.
+  inversion X0. subst.
+  apply (SPUF._u_mem _ (existT _ fx (inr s))).
+  destruct (excluded_middle_informative (fx = fx)).
+  - rewrite <- eq_rect_eq.
+    destruct ((SSPF.emb (B fx)) X X1); inversion EQ. auto.
+  - destruct n. auto.
+Defined.
+Next Obligation.
+  unfold depsum_embed in X0.
+  inversion X0. subst.
+  destruct s. destruct s.
+  - destruct (excluded_middle_informative (fx = x0)); inversion EQ.
+  - destruct (excluded_middle_informative (fx = x0)); subst; simpl.
+    + rewrite <- eq_rect_eq in EQ.
+      apply SSPF.mem_nat2.
+      apply (SPUF._u_mem _ s).
+      destruct (SSPF.emb (B x0) X X1); inversion EQ. auto.
+    + inversion EQ.
+Defined.
+Next Obligation.
+Proof.
+  unfold depsum_embed, depsum_map, SPUF.map.
+  destruct X0;
+  destruct (excluded_middle_informative (x = s)); auto.
+  destruct e. simpl.
+  rewrite SSPF.map_nat. unfold SPUF.map.
+  destruct ((SSPF.emb (B x)) X X1); auto.
+Defined.
+Next Obligation.
+  unfold depsum_embed; split; intros.
+  - dependent destruction H.
+    apply SSPF.eq_nat in H. inversion H.
+    split; intros; dependent destruction s; dependent destruction s; subst.
+    + destruct (excluded_middle_informative (fx2 = x)); tauto.
+    + split; intros;
+      destruct (excluded_middle_informative (fx2 = x)); auto;
+      destruct (SSPF.emb (B x) X (eq_rect fx2 (fun y : A => (B y) X) X1 x e0)) eqn : EQ1;        
+      destruct (SSPF.emb (B x) X (eq_rect fx2 (fun y : A => (B y) X) X0 x e0)) eqn : EQ2; inversion H2; subst;
+      replace (eq_rect x (fun y : A => (B y) X) X1 x eq_refl) with X1 in EQ1;
+      replace (eq_rect x (fun y : A => (B y) X) X0 x eq_refl) with X0 in EQ2;
+      try (apply H0 in EQ1; rewrite EQ1 in EQ2; inversion EQ2);
+      try (apply H0 in EQ2; rewrite EQ1 in EQ2; inversion EQ2);
+      try (rewrite <- eq_rect_eq; auto); auto.
+    + destruct (excluded_middle_informative (fx2 = x)); inversion H2.
+    + destruct (excluded_middle_informative (fx2 = x)); subst.
+      replace (eq_rect x (fun y : A => (B y) X) X1 x eq_refl) with X1 in H2;
+      replace (eq_rect x (fun y : A => (B y) X) X0 x eq_refl) with X0 in H3.
+      destruct (SSPF.emb (B x) X X0 s) eqn : EQ1;
+      destruct (SSPF.emb (B x) X X1 s) eqn : EQ2; inversion H3; inversion H2; subst.
+      apply (H1 _ _ _ EQ2 EQ1).
+      { rewrite <- eq_rect_eq; auto. }
+      { rewrite <- eq_rect_eq; auto. }
+      { rewrite <- eq_rect_eq; auto. }
+      inversion H2.
+  - destruct H.
+    assert (fx2 = fx1).
+    { specialize (H (existT _ fx2 (inl tt) : {a : A & (unit + SSPF.Sh (B a))%type}) 
+                    (inl false)). simpl in H.
+      destruct (excluded_middle_informative (fx1 = fx2)); auto.
+      destruct (excluded_middle_informative (fx2 = fx2)).
+      - destruct H. specialize (H eq_refl). inversion H.
+      - destruct n0; auto. } subst.
+    constructor. apply SSPF.eq_nat.
+    split; intros.
+    + split; intros.
+      * clear H0.
+        specialize (H (existT _ fx1 (inr s) : {a : A & (unit + SSPF.Sh (B a))%type})
+                   (inr (existT _ fx1 e))). simpl in H.
+        destruct (excluded_middle_informative (fx1 = fx1)).
+        replace (eq_rect fx1 (fun y : A => (B y) X) X1 fx1 e0) with X1 in H.
+        replace (eq_rect fx1 (fun y : A => (B y) X) X0 fx1 e0) with X0 in H.
+        rewrite H1 in H. destruct H. specialize (H eq_refl).
+        destruct (SSPF.emb (B fx1) X X0 s); inversion H.
+        dependent destruction H3. auto.
+        { rewrite <- eq_rect_eq. auto. }
+        { rewrite <- eq_rect_eq. auto. }
+        destruct n; auto.
+      * clear H0.
+        specialize (H (existT _ fx1 (inr s) : {a : A & (unit + SSPF.Sh (B a))%type})
+                   (inr (existT _ fx1 e))). simpl in H.
+        destruct (excluded_middle_informative (fx1 = fx1)).
+        replace (eq_rect fx1 (fun y : A => (B y) X) X1 fx1 e0) with X1 in H.
+        replace (eq_rect fx1 (fun y : A => (B y) X) X0 fx1 e0) with X0 in H.
+        rewrite H1 in H. destruct H. specialize (H0 eq_refl).
+        destruct (SSPF.emb (B fx1) X X1 s); inversion H0.
+        dependent destruction H3. auto.
+        { rewrite <- eq_rect_eq. auto. }
+        { rewrite <- eq_rect_eq. auto. }
+        destruct n; auto.
+    + clear H.
+      specialize (H0 (existT _ fx1 (inr s) : {a : A & (() + SSPF.Sh (B a))%type}) 
+                     x1 x2). simpl in H0.
+      destruct (excluded_middle_informative (fx1 = fx1)).
+      replace (eq_rect fx1 (fun y : A => (B y) X) X1 fx1 e) with X1 in H0.
+      replace (eq_rect fx1 (fun y : A => (B y) X) X0 fx1 e) with X0 in H0.
+      rewrite H1 in H0. rewrite H2 in H0.
+      apply H0; auto.
+      { rewrite <- eq_rect_eq. auto. }
+      { rewrite <- eq_rect_eq. auto. }
+      destruct n; auto.
+Qed.
+Next Obligation.
+  unfold depsum_embed in EQ.
+  assert (H:= equal_f EQ (existT _ m (inl tt))). simpl in H.
+  destruct (excluded_middle_informative (m = m));
+  destruct (excluded_middle_informative (n = m)); inversion H; subst.
+  - f_equal. apply SSPF.inj. extensionality s.
+    apply equal_f with (x:= (existT _ m (inr s))) in EQ.
+    destruct (excluded_middle_informative (m = m)).
+    + replace (eq_rect m (fun y : A => (B y) X) X1 m e0) with X1 in EQ.
+      replace (eq_rect m (fun y : A => (B y) X) X0 m e0) with X0 in EQ.
+      destruct (SSPF.emb (B m) X X1),(SSPF.emb (B m) X X0); inversion EQ; auto.      
+      dependent destruction H1. auto.
+      { rewrite <- eq_rect_eq. auto. }
+      { rewrite <- eq_rect_eq. auto. }
+    + destruct n. auto.
+  - destruct n0. auto.
+Defined.
+
+End Dependent_sum_SSPF.
+
+Section Option_SSPF.
+
+Definition opt_mem X (x: option X) : X -> Type :=
+  match x with
+  | None => (fun y => False)
+  | Some x' => eq x' end.
+
+Inductive opt_eq (X : Type) (EQ: X -> X -> Prop) : option X -> option X -> Prop :=
+  | _opt_eq_none : opt_eq EQ None None
+  | _opt_eq_some x1 x2 : EQ x1 x2 -> opt_eq EQ (Some x1) (Some x2).
+
+Definition opt_uni X Y (x: option X) (ALL: forall y, opt_mem x y -> Y)
+  : option Y.
+  destruct x.
+  - apply (Some (ALL _ (eq_refl x))).
+  - apply None.
+Defined.
+
+Program Definition opt_Fn :=
+  (@PFunctor.mk_data option opt_mem opt_eq option_map opt_uni _).
+Next Obligation.
+Proof.
+  unfold option_map. destruct a; unfold opt_uni.
+  - rewrite INV. auto.
+  - auto.
+Defined.
+
+Definition opt_embed X (x: option X) (s: unit) :=
+  match x with
+  | Some x' => inl x'
+  | None => inr tt
+  end.
+
+Program Definition Option_sspf : SSPF.t := 
+  @SSPF.mk opt_Fn _ _ opt_embed _ _ _ _ _.
+Next Obligation.
+  unfold opt_embed. destruct fx; inversion X0.
+  - apply (SPUF._u_mem _ tt). auto.
+Defined.
+Next Obligation.
+  unfold opt_embed in X0. inversion X0. subst.
+  destruct fx; inversion EQ.
+  constructor.
+Defined.
+Next Obligation.
+  destruct x; auto.
+Defined.
+Next Obligation.
+  unfold opt_embed; split; intros.
+  - inversion H; split; intros.
+    + tauto.
+    + inversion H2.
+    + split; intro; inversion H3.
+    + inversion H3. inversion H4. subst. auto.
+  - inversion H. destruct fx1, fx2.
+    + constructor. apply (H1 tt); auto.
+    + destruct (H0 tt tt). specialize (H3 eq_refl). inversion H3.
+    + destruct (H0 tt tt). specialize (H2 eq_refl). inversion H2.
+    + constructor.
+Defined.
+Next Obligation.
+Proof.
+  apply equal_f with tt in EQ.
+  destruct m, n; inversion EQ; auto.
+Qed.
+
+End Option_SSPF.
+
 
 Section Composition_SSPF.
 
 Variable F G: SSPF.t.
-
-Definition comp_map X Y (f: X -> Y) (x: F (G X)) :=
-  F.(PFunctor.map) (G.(PFunctor.map) f) x.
-
-Inductive comp_rel X : X -> F (G X) -> Prop :=
-| _comp_rel x gx fgx (HG : G.(PFunctor.rel) x gx) (HF : F.(PFunctor.rel) gx fgx) :
-    comp_rel x fgx.
-
-Definition comp_Fn := (PFunctor.mk_data (fun X => F (G X)) comp_map comp_rel).
 
 Definition comp_embed' X (x': F.(SSPF.Sh) -> (sum (G.(SSPF.Sh) ->
                                                  (sum X G.(SSPF.Ext))) F.(SSPF.Ext)))
@@ -362,105 +811,351 @@ Proof.
     rewrite H1 in H. rewrite H2 in H. inversion H. eauto.
 Qed.
 
-Lemma comp_embed'_pullback m (H: forall s x, ~ comp_embed' m s = inl x) :
-  exists m', m = SPUF.map F.(SSPF.Sh) F.(SSPF.Ext)
-                          (SPUF.map G.(SSPF.Sh) G.(SSPF.Ext) (False_rect unit)) m'.
-Proof.
-  unfold comp_embed', SPUF.map in *.
-  assert (EX : forall sf,
-             exists (xg: sum (G.(SSPF.Sh) -> sum False (G.(SSPF.Ext))) F.(SSPF.Ext)),
-               match m sf with
-               | inr ef => xg = inr ef
-               | inl ug =>
-                 exists xg', xg = inl xg' /\ forall sg,
-                 (match ug sg with
-                 | inr eg => xg' sg = inr eg
-                 | inl _ => True end) end).
-  { intros.
-    destruct (m sf) eqn : EQ.
-    - assert (EX : forall sg, exists (xg': False + SSPF.Ext G),
-             match s sg with
-             | inl _ => True
-             | inr eg => xg' = inr eg end).
-      { intros.
-        specialize (H (inr sg, sf)). simpl in H. rewrite EQ in H.
-        destruct (s sg). 
-        - exfalso. apply (H u). auto.
-        - eauto.
-      }
-      apply choice in EX. destruct EX. exists (inl x).
-      exists x.
-      split. auto. apply H0.
-    - eauto.
-  }
-  apply choice in EX. destruct EX.
-  exists x.
-  extensionality sf. specialize (H0 sf).
-  - destruct (m sf) eqn: EQ.
-    destruct H0. destruct H0.
-    rewrite H0. f_equal.
-    extensionality sg. specialize (H1 sg).
-    specialize (H (inr sg, sf)). simpl in H.
-    rewrite EQ in H. destruct (s sg).
-    + exfalso. apply (H u). auto.
-    + rewrite H1. auto.
-    + rewrite H0. auto.
-Qed.  
-
 Definition comp_embed X (x: F (G X)) :=
   comp_embed' (F.(SSPF.emb) _ (F.(PFunctor.map) (G.(SSPF.emb) X) x)).
 
 Program Definition Comp : SSPF.t := 
-  @SSPF.mk comp_Fn _ _ (PNatTrans.mk _ _ comp_embed _ _) _ _.
+  @SSPF.mk (comp_Fn F G) _ _ comp_embed _ _ _ _ _.
 Next Obligation.
-  extensionality s. destruct s; destruct s;
-  unfold SPUF.map, comp_embed;
-  repeat rewrite PNatTrans.map_nat; simpl;
-  unfold comp_map, SPUF.map; rewrite PNatTrans.map_nat; simpl;  
-  destruct ((SSPF.emb F) (G X) x); eauto.
-  rewrite PNatTrans.map_nat. simpl.
-  destruct ((SSPF.emb G) X f0); eauto.
-Qed.
+  unfold comp_embed, comp_embed'.
+  inversion X0. subst.
+  apply F.(SSPF.mem_nat1) in HF.
+  apply G.(SSPF.mem_nat1) in HG.
+  inversion HG. inversion HF. subst.
+  apply (SPUF._u_mem _ (inr s, s0)).
+  repeat rewrite SSPF.map_nat. simpl. unfold SPUF.map.
+  destruct ((SSPF.emb F) (G X) fx); inversion EQ0.
+  destruct ((SSPF.emb G) X gx); inversion EQ. auto.
+Defined.
 Next Obligation.
-  unfold comp_embed, comp_embed'. split; intros.
-  - inversion H. subst.
-    apply (PNatTrans.rel_nat F.(SSPF.emb)) in HF.
-    apply (PNatTrans.rel_nat G.(SSPF.emb)) in HG.
-    inversion HG. inversion HF. subst.
-    apply (SPUF._u_rel _ (inr s, s0)).
-    repeat rewrite (PNatTrans.map_nat). simpl. unfold SPUF.map.
-    destruct ((SSPF.emb F) (G X) fx); inversion EQ0.
-    destruct ((SSPF.emb G) X gx); inversion EQ. auto.
-  - inversion H; clear H. subst.
-    repeat rewrite (PNatTrans.map_nat) in EQ. simpl in EQ. unfold SPUF.map in EQ.
-    destruct s. destruct s.
-    + destruct ((SSPF.emb F) (G X) fx); inversion EQ.
-    + destruct ((SSPF.emb F) (G X) fx) eqn : H; inversion EQ.
-      destruct ((SSPF.emb G) X f) eqn: H2; inversion EQ. subst. clear H1 EQ.
-      apply (_comp_rel _ f).
-      apply (PNatTrans.rel_nat G.(SSPF.emb)). simpl. apply (SPUF._u_rel _ s H2).
-      apply (PNatTrans.rel_nat F.(SSPF.emb)). simpl. apply (SPUF._u_rel _ s0 H).
-Qed.
+  unfold comp_embed, comp_embed' in X0.
+  inversion X0. clear X0. subst.
+  destruct s. destruct s;
+  repeat rewrite SSPF.map_nat in EQ; unfold SPUF.map in EQ;
+  destruct ((SSPF.emb F) (G X) fx) eqn: H1; inversion EQ.
+  destruct ((SSPF.emb G) X f) eqn: H2; inversion EQ. subst.
+  apply (_comp_mem F G _ f).
+  apply G.(SSPF.mem_nat2). simpl. apply (SPUF._u_mem _ s H2).
+  apply F.(SSPF.mem_nat2). simpl. apply (SPUF._u_mem _ s0 H1).
+Defined.
 Next Obligation.
-  apply comp_embed'_pullback in CONST.
-  destruct CONST.
-  apply SSPF.embedded_pullback in H. destruct H.
-  apply (SSPF.preserve_pullback F (@SSPF.embedded_pullback _ _ _ _)) in H.
-  destruct H. exists x1.
-  subst. unfold comp_map.
-  repeat f_equal. extensionality s. destruct s.
+  destruct s;
+  unfold SPUF.map, comp_embed, comp_map, comp_embed';
+  repeat rewrite SSPF.map_nat; unfold SPUF.map;
+  rewrite SSPF.map_nat; unfold SPUF.map;
+  destruct (SSPF.emb F (G X) x); auto.
+  rewrite SSPF.map_nat; unfold SPUF.map.
+  destruct (SSPF.emb G X f0); auto.
+Defined.
+Next Obligation.
+  unfold comp_embed, comp_eq, comp_embed'. split; intros.
+  - split; intros.
+    + split; intros; destruct s.
+      * destruct s.
+        --apply SSPF.eq_nat in H.
+          inversion H.
+          rewrite SSPF.map_nat. rewrite SSPF.map_nat in H0. unfold SPUF.map in *.
+          destruct (SSPF.emb F (G X) fx1) eqn : EQ1;
+          destruct (SSPF.emb F (G X) fx2) eqn : EQ2.
+          ++auto.
+          ++apply H1 in EQ2. simpl in *. rewrite EQ2 in EQ1. inversion EQ1.
+          ++apply H1 in EQ1. simpl in *. rewrite EQ2 in EQ1. inversion EQ1.
+          ++apply H1 in EQ1. simpl in *. rewrite EQ2 in EQ1. inversion EQ1.
+            symmetry. auto.
+        --repeat rewrite SSPF.map_nat in *. unfold SPUF.map in *.
+          apply SSPF.eq_nat in H. inversion H.
+          destruct (SSPF.emb F (G X) fx1) eqn : EQ1;
+          destruct (SSPF.emb F (G X) fx2) eqn : EQ2.
+
+          destruct (SSPF.emb G X f) eqn : EQ3;
+          destruct (SSPF.emb G X f0) eqn : EQ4; inversion H0;
+          specialize (H2 _ _ _ EQ1 EQ2); apply SSPF.eq_nat in H2; inversion H2.
+          ++apply H3 in EQ3. rewrite EQ3 in EQ4. inversion EQ4.
+          ++apply H3 in EQ3. rewrite EQ3 in EQ4. inversion EQ4. auto.
+
+          ++destruct (SSPF.emb G X f); inversion H0.
+            apply H1 in EQ2. simpl in *. rewrite EQ1 in EQ2. inversion EQ2.
+          ++apply H1 in EQ1. simpl in *. rewrite EQ1 in EQ2. inversion EQ2.
+          ++apply H1 in EQ1. simpl in *. rewrite EQ1 in EQ2. inversion EQ2. auto.
+      * destruct s.
+        --repeat rewrite SSPF.map_nat in *. unfold SPUF.map in *.
+          apply SSPF.eq_nat in H. destruct H.
+          destruct (SSPF.emb F (G X) fx1) eqn : EQ1;
+          destruct (SSPF.emb F (G X) fx2) eqn : EQ2; inversion H0; auto.
+          ++apply H in EQ2. simpl in *. rewrite EQ2 in EQ1. inversion EQ1.
+          ++apply H in EQ1. simpl in *. rewrite EQ2 in EQ1. inversion EQ1.
+          ++apply H in EQ2. simpl in *. rewrite EQ2 in EQ1. inversion EQ1. auto.
+        --repeat rewrite SSPF.map_nat in *. unfold SPUF.map in *.
+          apply SSPF.eq_nat in H. destruct H.
+          destruct (SSPF.emb F (G X) fx1) eqn : EQ1;
+          destruct (SSPF.emb F (G X) fx2) eqn : EQ2.
+          ++specialize (H1 _ _ _ EQ1 EQ2). apply SSPF.eq_nat in H1. destruct H1.
+            destruct (SSPF.emb G X f0) eqn : EQ3;
+            destruct (SSPF.emb G X f) eqn : EQ4; inversion H0.
+            **apply H1 in EQ3. rewrite EQ3 in EQ4. inversion EQ4.
+            **apply H1 in EQ3. rewrite EQ3 in EQ4. inversion EQ4. auto.
+          ++apply H in EQ2. simpl in *. rewrite EQ2 in EQ1. inversion EQ1.
+          ++apply H in EQ1. simpl in *. rewrite EQ2 in EQ1. inversion EQ1.
+          ++apply H in EQ2. simpl in *. rewrite EQ2 in EQ1. inversion EQ1. auto.
+    + destruct s. repeat rewrite SSPF.map_nat in *. unfold SPUF.map in *.
+      repeat rewrite SSPF.map_nat in *. apply SSPF.eq_nat in H. destruct H.
+      destruct s.
+      * destruct (SSPF.emb F (G X) fx1) eqn : EQ1;
+        destruct (SSPF.emb F (G X) fx2) eqn : EQ2; inversion H0; inversion H1.
+      * destruct (SSPF.emb F (G X) fx1) eqn : EQ1;
+        destruct (SSPF.emb F (G X) fx2) eqn : EQ2; inversion H0; inversion H1.
+        specialize (H2 _ _ _ EQ1 EQ2). apply SSPF.eq_nat in H2. destruct H2.
+        destruct (SSPF.emb G X f s) eqn : EQ3;
+        destruct (SSPF.emb G X f0 s) eqn : EQ4; inversion H4; inversion H5.
+        subst. apply (H3 _ _ _ EQ3 EQ4).
+  - apply SSPF.eq_nat. destruct H. split; intros.
+    + split; intros;
+      specialize (H (inl tt, s) (inr (inr e))); simpl in *; clear H0;
+      repeat rewrite SSPF.map_nat in H; unfold SPUF.map in H;
+      rewrite H1 in H; destruct H.
+      * specialize (H eq_refl);
+        destruct (SSPF.emb F (G X) fx2 s); inversion H. auto.
+      * specialize (H0 eq_refl);
+        destruct (SSPF.emb F (G X) fx1 s); inversion H0. auto.
+    + apply SSPF.eq_nat. split; intros.
+      * split; intros;
+        specialize (H (inr s0, s) (inr (inl e))); simpl in *; clear H0;
+        repeat rewrite SSPF.map_nat in H; unfold SPUF.map in H;
+        rewrite H1 in H; rewrite H2 in H; rewrite H3 in H;
+        destruct H.
+        -- specialize (H eq_refl);
+           destruct (SSPF.emb G X x2 s0); inversion H. auto.
+        -- specialize (H0 eq_refl).
+           destruct (SSPF.emb G X x1 s0); inversion H0. auto.
+      * specialize (H0 (inr s0, s) x0 x3). simpl in *. clear H.
+        repeat rewrite SSPF.map_nat in H0. unfold SPUF.map in H0.
+        rewrite H1 in H0. rewrite H2 in H0. rewrite H3 in H0. rewrite H4 in H0.
+        apply H0; auto.
 Qed.
 Next Obligation.
   unfold comp_embed in EQ.
   apply comp_embed'_injective in EQ.
   apply SSPF.inj in EQ. apply SSPF.map_injective in EQ.
   apply EQ. apply SSPF.inj.
-Qed.
+Defined.
 
 End Composition_SSPF.
 
 
+Section Dependent_sum_dec_SSPF.
+
+Variable A: Type.
+Variable B: A -> SSPF.t.
+Variable eq_dec: forall (a1 a2 : A), {a1=a2} + {a1<>a2}.
+
+Definition depsum_dec_map X Y (f: X -> Y) (x: sigT (fun a => (B a) X))
+  : (sigT (fun a => (B a) Y)) :=
+  match x with
+  | existT _ a x' => existT _ a ((B a).(PFunctor.map) f x') end.
+
+Definition depsum_dec_mem X (x: sigT (fun a => (B a) X)) : X -> Type :=
+  match x with
+  | existT _ a x' => (B a).(PFunctor.mem) x' end.
+
+Inductive depsum_dec_eq X (EQ: X -> X -> Prop)
+  : (sigT (fun a => (B a) X)) -> (sigT (fun a => (B a) X)) -> Prop :=
+  | _depsum_dec_eq a fx1 fx2 : (B a).(PFunctor.eq) EQ fx1 fx2 -> 
+                         depsum_dec_eq EQ (existT _ a fx1) (existT _ a fx2).
+
+Definition depsum_dec_uni X Y (x: sigT (fun a => (B a) X))
+           (ALL: forall y, depsum_dec_mem x y -> Y) : (sigT (fun a => (B a) Y)).
+  destruct x.
+  apply (existT _ x ((B x).(PFunctor.uni) f (fun x0 r => ALL _ r))).
+Defined.
+
+Program Definition depsum_dec_Fn :=
+  (@PFunctor.mk_data (fun X => sigT (fun a => (B a) X)) depsum_dec_mem
+                     depsum_dec_eq depsum_dec_map depsum_dec_uni _).
+Next Obligation.
+Proof.
+  unfold depsum_dec_map. unfold depsum_dec_uni.
+  f_equal. apply (B a).(PFunctor.uni_correct).
+  intros. apply INV.
+Defined.
+
+Definition depsum_dec_embed X (x: sigT (fun a => (B a) X))
+           (s: sigT (fun a => sum unit (B a).(SSPF.Sh))) :
+  sum X (sum bool (sigT (fun a => (B a).(SSPF.Ext)))) :=
+match x with
+| existT _ a x' =>
+  match s with
+  | existT _ a' sh =>
+    match (eq_dec a a') with
+    | left pf =>
+      match sh with
+      | inl _ => inr (inl true)
+      | inr sh' =>
+        match (B a').(SSPF.emb) _ (eq_rect _ (fun y => (B y) X) x' _ pf) sh' with
+        | inl a => inl a
+        | inr b => inr (inr (existT _ a' b)) end
+      end
+    | right _ => inr (inl false)
+    end
+  end
+end.
+
+Program Definition Depend_dec_Sum : SSPF.t :=
+  @SSPF.mk depsum_dec_Fn _ _ depsum_dec_embed _ _ _ _ _.
+Next Obligation.
+  unfold depsum_dec_embed. simpl in X0.
+  apply (B fx).(SSPF.mem_nat1) in X0.
+  inversion X0. subst.
+  apply (SPUF._u_mem _ (existT _ fx (inr s))).
+  destruct (eq_dec fx fx).
+  - rewrite <- (eq_rect_eq_dec eq_dec).
+    destruct ((SSPF.emb (B fx)) X X1); inversion EQ. auto.
+  - destruct n. auto.
+Defined.
+Next Obligation.
+  unfold depsum_dec_embed in X0.
+  inversion X0. subst.
+  destruct s. destruct s.
+  - destruct (eq_dec fx x0); inversion EQ.
+  - destruct (eq_dec fx x0); subst; simpl.
+    + rewrite <- (eq_rect_eq_dec eq_dec) in EQ.
+      apply SSPF.mem_nat2.
+      apply (SPUF._u_mem _ s).
+      destruct (SSPF.emb (B x0) X X1); inversion EQ. auto.
+    + inversion EQ.
+Defined.
+Next Obligation.
+Proof.
+  unfold depsum_dec_embed, depsum_dec_map, SPUF.map.
+  destruct X0;
+  destruct (eq_dec x s); auto.
+  destruct e. simpl.
+  rewrite SSPF.map_nat. unfold SPUF.map.
+  destruct ((SSPF.emb (B x)) X X1); auto.
+Defined.
+Next Obligation.
+  unfold depsum_dec_embed; split; intros.
+  - dependent destruction H.
+    apply SSPF.eq_nat in H. inversion H.
+    split; intros; dependent destruction s; dependent destruction s; subst.
+    + destruct (eq_dec fx2 x); tauto.
+    + split; intros;
+      destruct (eq_dec fx2 x); auto;
+      destruct (SSPF.emb (B x) X (eq_rect fx2 (fun y : A => (B y) X) X1 x e0)) eqn : EQ1;        
+      destruct (SSPF.emb (B x) X (eq_rect fx2 (fun y : A => (B y) X) X0 x e0)) eqn : EQ2; inversion H2; subst;
+      replace (eq_rect x (fun y : A => (B y) X) X1 x eq_refl) with X1 in EQ1;
+      replace (eq_rect x (fun y : A => (B y) X) X0 x eq_refl) with X0 in EQ2;
+      try (apply H0 in EQ1; rewrite EQ1 in EQ2; inversion EQ2);
+      try (apply H0 in EQ2; rewrite EQ1 in EQ2; inversion EQ2);
+      try (rewrite <- (eq_rect_eq_dec eq_dec); auto); auto.
+    + destruct (eq_dec fx2 x); inversion H2.
+    + destruct (eq_dec fx2 x); subst.
+      replace (eq_rect x (fun y : A => (B y) X) X1 x eq_refl) with X1 in H2;
+      replace (eq_rect x (fun y : A => (B y) X) X0 x eq_refl) with X0 in H3.
+      destruct (SSPF.emb (B x) X X0 s) eqn : EQ1;
+      destruct (SSPF.emb (B x) X X1 s) eqn : EQ2; inversion H3; inversion H2; subst.
+      apply (H1 _ _ _ EQ2 EQ1).
+      { rewrite <- (eq_rect_eq_dec eq_dec); auto. }
+      { rewrite <- (eq_rect_eq_dec eq_dec); auto. }
+      { rewrite <- (eq_rect_eq_dec eq_dec); auto. }
+      inversion H2.
+  - destruct H.
+    assert (fx2 = fx1).
+    { specialize (H (existT _ fx2 (inl tt) : {a : A & (unit + SSPF.Sh (B a))%type}) 
+                    (inl false)). simpl in H.
+      destruct (eq_dec fx1 fx2); auto.
+      destruct (eq_dec fx2 fx2).
+      - destruct H. specialize (H eq_refl). inversion H.
+      - destruct n0; auto. } subst.
+    constructor. apply SSPF.eq_nat.
+    split; intros.
+    + split; intros.
+      * clear H0.
+        specialize (H (existT _ fx1 (inr s) : {a : A & (unit + SSPF.Sh (B a))%type})
+                   (inr (existT _ fx1 e))). simpl in H.
+        destruct (eq_dec fx1 fx1).
+        replace (eq_rect fx1 (fun y : A => (B y) X) X1 fx1 e0) with X1 in H.
+        replace (eq_rect fx1 (fun y : A => (B y) X) X0 fx1 e0) with X0 in H.
+        rewrite H1 in H. destruct H. specialize (H eq_refl).
+        destruct (SSPF.emb (B fx1) X X0 s); inversion H.
+        dependent destruction H3. auto.
+        { rewrite <- (eq_rect_eq_dec eq_dec). auto. }
+        { rewrite <- (eq_rect_eq_dec eq_dec). auto. }
+        destruct n; auto.
+      * clear H0.
+        specialize (H (existT _ fx1 (inr s) : {a : A & (unit + SSPF.Sh (B a))%type})
+                   (inr (existT _ fx1 e))). simpl in H.
+        destruct (eq_dec fx1 fx1).
+        replace (eq_rect fx1 (fun y : A => (B y) X) X1 fx1 e0) with X1 in H.
+        replace (eq_rect fx1 (fun y : A => (B y) X) X0 fx1 e0) with X0 in H.
+        rewrite H1 in H. destruct H. specialize (H0 eq_refl).
+        destruct (SSPF.emb (B fx1) X X1 s); inversion H0.
+        dependent destruction H3. auto.
+        { rewrite <- (eq_rect_eq_dec eq_dec). auto. }
+        { rewrite <- (eq_rect_eq_dec eq_dec). auto. }
+        destruct n; auto.
+    + clear H.
+      specialize (H0 (existT _ fx1 (inr s) : {a : A & (() + SSPF.Sh (B a))%type}) 
+                     x1 x2). simpl in H0.
+      destruct (eq_dec fx1 fx1).
+      replace (eq_rect fx1 (fun y : A => (B y) X) X1 fx1 e) with X1 in H0.
+      replace (eq_rect fx1 (fun y : A => (B y) X) X0 fx1 e) with X0 in H0.
+      rewrite H1 in H0. rewrite H2 in H0.
+      apply H0; auto.
+      { rewrite <- (eq_rect_eq_dec eq_dec). auto. }
+      { rewrite <- (eq_rect_eq_dec eq_dec). auto. }
+      destruct n; auto.
+Qed.
+Next Obligation.
+  unfold depsum_dec_embed in EQ.
+  assert (H:= equal_f EQ (existT _ m (inl tt))). simpl in H.
+  destruct (eq_dec m m);
+  destruct (eq_dec n m); inversion H; subst.
+  - f_equal. apply SSPF.inj. extensionality s.
+    apply equal_f with (x:= (existT _ m (inr s))) in EQ.
+    destruct (eq_dec m m).
+    + replace (eq_rect m (fun y : A => (B y) X) X1 m e0) with X1 in EQ.
+      replace (eq_rect m (fun y : A => (B y) X) X0 m e0) with X0 in EQ.
+      destruct (SSPF.emb (B m) X X1),(SSPF.emb (B m) X X0); inversion EQ; auto.
+      apply (inj_pair2_eq_dec _ eq_dec) in H1. subst. auto.
+      { rewrite <- (eq_rect_eq_dec eq_dec). auto. }
+      { rewrite <- (eq_rect_eq_dec eq_dec). auto. }
+    + destruct n. auto.
+  - destruct n0. auto.
+Defined.
+
+End Dependent_sum_dec_SSPF.
+
 Section List_SSPF.
+
+Fixpoint list_mem X (l: list X) (x: X) : Type :=
+  match l with
+  | nil => False
+  | cons hd tl => eq hd x + list_mem tl x end.
+
+Inductive list_eq (X : Type) (EQ: X -> X -> Prop) : list X -> list X -> Prop :=
+  | _list_eq_nil : list_eq EQ nil nil
+  | _list_eq_cons hd1 hd2 tl1 tl2 (HD: EQ hd1 hd2) (TL: list_eq EQ tl1 tl2) : 
+      (list_eq EQ (cons hd1 tl1) (cons hd2 tl2)).
+
+Definition list_uni X Y (x: list X) (ALL: forall y, list_mem x y -> Y) : list Y.
+  induction x.
+  - apply nil.
+  - apply cons.
+    + apply (ALL a (inl (eq_refl a))).
+    + apply IHx. intros.
+      apply (ALL y (inr X0)).
+Defined.
+
+Definition list_uni_correct : forall X Y (a: list X) (ALL: forall x, list_mem a x -> Y)
+                       (f: Y -> X) (INV: forall x r, f (ALL x r) = x),
+    List.map f (list_uni _ ALL) = a.
+Proof.
+  intros. induction a.
+  - auto.
+  - simpl. f_equal.
+    + apply INV.
+    + apply IHa. intros. apply INV.
+Defined.
 
 Fixpoint list_embed X (l: list X) (s: list unit) : X + unit :=
   match l with
@@ -473,41 +1168,82 @@ Fixpoint list_embed X (l: list X) (s: list unit) : X + unit :=
       end
   end.
 
-(* @jeehoonkang: naming: List? FList? ... *)
 Program Definition List_sspf : SSPF.t := 
-  @SSPF.mk (PFunctor.mk_data list List.map List.In) (list unit) unit 
-          (PNatTrans.mk _ _ list_embed _ _) _ _.
+  @SSPF.mk (PFunctor.mk_data list list_mem list_eq List.map list_uni 
+                             list_uni_correct) _ _ list_embed _ _ _ _ _.
 Next Obligation.
-  induction x; eauto.
-  extensionality s. simpl. rewrite IHx.
-  destruct s; eauto.
-  destruct s; eauto.
+  induction fx; inversion X0; subst.
+  - apply (SPUF._u_mem _ (cons tt nil)). auto.
+  - apply IHfx in X1.
+    inversion X1. subst.
+    apply (SPUF._u_mem _ (cons tt s)).
+    destruct s.
+    + destruct fx; inversion EQ.
+    + auto.
+Defined.
+Next Obligation. 
+  induction fx; inversion X0; subst.
+  - inversion EQ.
+  - destruct s; inversion EQ. destruct s; inversion EQ.
+    + repeat constructor.
+    + apply inr. apply IHfx.
+      apply (SPUF._u_mem _ (cons u0 s) EQ).
+Defined.
+Next Obligation.
+  revert s.
+  induction x; auto.
+  intros. destruct s; auto. destruct s; auto.
+  unfold SPUF.map in *. simpl.
+  apply (IHx (cons u0 s)).
+Defined.
+Next Obligation.
+  revert fx2. induction fx1; intros; split; intros.
+  - inversion H. subst. unfold list_embed. split; intros.
+    + tauto.
+    + inversion H0.
+  - destruct fx2. constructor. destruct H.
+    specialize (H (cons tt nil) tt). unfold list_embed in H.
+    destruct H. specialize (H eq_refl). inversion H.
+  - inversion H. subst. clear H.
+    split; intros; apply (IHfx1 tl2) in TL; destruct TL.
+    + split; (intros; simpl in *;
+      destruct s; [auto | ]; destruct s; [inversion H1| ]);
+      apply H; auto.
+    + destruct s. simpl in *. inversion H.
+      simpl in *. destruct s. inversion H. inversion H0. subst. auto.
+      apply (H2 _ _ _ H H0).
+  - destruct H. destruct fx2.
+    + specialize (H (cons tt nil) tt). destruct H.
+      simpl in H1. specialize (H1 eq_refl). inversion H1.
+    + specialize (IHfx1 fx2). destruct IHfx1.
+      constructor.
+      specialize (H0 (cons tt nil)). simpl in H0.
+      apply H0; auto.
+      
+      apply H2.
+      split; intros.
+      * split; intros;
+        specialize (H (cons tt s) tt); simpl in H;
+        destruct s.
+        -- destruct fx1. simpl in H3. inversion H3.
+           destruct fx2. simpl. auto.
+           simpl. auto.
+           simpl in H3.
+           destruct fx2. auto. auto.
+        -- destruct e. apply H. auto.
+        -- destruct fx2. simpl in H3. inversion H3.
+           destruct fx1. simpl. auto.
+           simpl. auto.
+           simpl in H3.
+           destruct fx1. auto. simpl. auto.
+        -- destruct e. apply H. auto.
+      * specialize (H0 (cons tt s) x1 x2). simpl in H0.
+        destruct s. 
+        destruct fx1. inversion H3. inversion H3.
+        apply (H0 H3 H4).
 Qed.
 Next Obligation.
-  split; intros.
-  - induction fx; destruct H.
-    + subst. apply (SPUF._u_rel _ (cons tt nil)). eauto.
-    + apply IHfx in H.
-      inversion H. subst.
-      apply (SPUF._u_rel _ (cons tt s)). simpl.
-      destruct s.
-      * destruct fx; inversion EQ.
-      * auto.
-  - induction fx.
-    + inversion H. subst. inversion EQ.
-    + inversion H. subst.
-      destruct s; inversion EQ. destruct s; inversion EQ.
-      * subst. simpl. auto.
-      * simpl. right.
-        apply IHfx.
-        apply (SPUF._u_rel _ (cons u0 s) EQ).
-Qed.
-Next Obligation.
-  destruct m.
-  - exists nil. eauto.
-  - exfalso. eapply (CONST (cons () nil)); simpl; eauto.
-Qed.
-Next Obligation.
+Proof.
   assert (EQ' := equal_f EQ). clear EQ.
   revert n EQ'. induction m; intros.
   - destruct n; eauto. 
@@ -519,309 +1255,65 @@ Next Obligation.
       * intros. specialize (EQ' (cons tt x0)). 
         destruct x0; eauto.
         destruct m, n; eauto.
-Qed.
+Defined.
 
 End List_SSPF.
+
+
+Section Embedded_SSPF.
+
+Variable F: PFunctor.t_data.
+Variable G: SSPF.t.
+Variable Nt: PNatTrans.t F G.
+Hypothesis inj: forall X (m n: F X) (EQ: Nt _ m = Nt _ n), m = n.
+
+Definition embedded_embed X (x : F X) := G.(SSPF.emb) _ (Nt _ x).
+
+Program Definition Embedded_sspf : SSPF.t := 
+  @SSPF.mk F _ _ embedded_embed _ _ _ _ _.
+Next Obligation.
+Proof.
+  apply G.(SSPF.mem_nat1), Nt.(PNatTrans.mem_nat1), X0.
+Defined.
+Next Obligation.
+Proof.
+  apply Nt.(PNatTrans.mem_nat2), G.(SSPF.mem_nat2), X0.
+Defined.
+Next Obligation.
+  unfold embedded_embed.
+  rewrite Nt.(PNatTrans.map_nat).
+  apply SSPF.map_nat.
+Defined.
+Next Obligation.
+  rewrite Nt.(PNatTrans.eq_nat).
+  apply SSPF.eq_nat.
+Qed.
+Next Obligation.
+  unfold embedded_embed in EQ.
+  apply SSPF.inj in EQ.
+  apply inj in EQ. auto.
+Qed.
+
+End Embedded_SSPF.
 
 (*
-Section List_SSPF.
+Definition U Sh Ext := Comp (Expn Sh) (Coprod Ident (Const Ext)).
 
-Fixpoint list_embed X (l: list X) (s: list unit) : X + unit :=
-  match l with
-  | nil => inr tt
-  | cons hd tl => 
-      match s with 
-      | cons _ nil => inl hd
-      | cons _ stl => list_embed tl stl
-      | _ => inr tt
-      end
-  end.
+Lemma mem_eq1 Sh Ext X (u: Sh -> X + Ext) (x: X)
+  : SPUF.u_mem u x -> (U Sh Ext).(PFunctor.mem) u x.
+Proof.
+  intro. inversion X0. subst. simpl.
+  apply (_comp_mem (Expn Sh) (Coprod Ident (Const Ext)) _ (inl x)).
+  - simpl. constructor.
+  - simpl. rewrite <- EQ. constructor.
+Defined.
 
-Inductive list_rel X : X -> list X -> Prop :=
-| _list_rel_hd x tl : list_rel x (cons x tl)
-| _list_rel_tl x hd tl (TL: list_rel x tl) : list_rel x (cons hd tl).
-
-Program Definition List_sspf : SSPF.t := 
-  @SSPF.mk (PFunctor.mk_data list List.map list_rel) (list unit) unit 
-          (PNatTrans.mk _ _ list_embed _ _) _ _.
-Next Obligation.
-  induction x; eauto.
-  extensionality s. simpl. rewrite IHx.
-  destruct s; eauto.
-  destruct s; eauto.
-Qed.
-Next Obligation.
-  split; intros.
-  - induction fx; inversion H; subst.
-    + apply (SPUF._u_rel _ (cons tt nil)). auto.
-    + apply IHfx in TL. clear IHfx. simpl.
-      inversion TL. subst.
-      apply (SPUF._u_rel _ (cons tt s)).
-      destruct s.
-      * destruct fx; simpl in EQ; inversion EQ.
-      * auto.
-  - induction fx.
-    + inversion H. subst. inversion EQ.
-    + inversion H. subst.
-      simpl in EQ.
-      destruct s; inversion EQ. destruct s; inversion EQ.
-      * subst. constructor.
-      * constructor.
-        apply IHfx.
-        apply (SPUF._u_rel _ (cons u0 s) EQ).
-Qed.
-Next Obligation.
-  destruct m.
-  - exists nil. eauto.
-  - exfalso. eapply (CONST (cons () nil)); simpl; eauto.
-Qed.
-Next Obligation.
-  assert (EQ' := equal_f EQ). clear EQ.
-  revert n EQ'. induction m; intros.
-  - destruct n; eauto. 
-    specialize (EQ' (cons tt nil)). inversion EQ'.
-  - destruct n.
-    + specialize (EQ' (cons tt nil)). inversion EQ'.
-    + rewrite (IHm n).
-      * specialize (EQ' (cons tt nil)). inversion EQ'; subst; auto.
-      * intros. specialize (EQ' (cons tt x0)). 
-        destruct x0; eauto.
-        destruct m, n; eauto.
-Qed.
-
-End List_SSPF.
+Lemma mem_eq2 Sh Ext X (u: Sh -> X + Ext) (x: X)
+  : (U Sh Ext).(PFunctor.mem) u x -> SPUF.u_mem u x.
+Proof.
+  intro. inversion X0. subst. simpl in *.
+  destruct gx; inversion HG. subst.
+  inversion HF. subst.
+  econstructor. apply H1.
+Defined.
 *)
-
-Section Dependent_function_SSPF.
-
-Variable A: Type.
-Variable B: A -> SSPF.t.
-(* @jeehoonkang: excluded_middle_informative is strong; use A's decidability. *)
-
-Definition depfun_map X Y (f: X -> Y) (x: forall a : A, B a X) :=
-  fun (a: A) => (B a).(PFunctor.map) f (x a).
-
-Inductive depfun_rel X : X -> (forall a : A, B a X) -> Prop :=
-| _depfun_rel x a f (RE: (B a).(PFunctor.rel) x (f a)) : depfun_rel x f.
-
-Definition depfun_Fn :=
-  (PFunctor.mk_data (fun X => forall a: A, B a X) depfun_map depfun_rel).
-
-Definition depfun_embed X (x: forall a : A, B a X) (s: SSPF.dep_sum B (SSPF.Sh)) : (X + (SSPF.dep_sum B (SSPF.Ext))) :=
-  match s with
-  | SSPF.dep _ _ a sh =>
-    match (B a).(SSPF.emb) _ (x a) sh with
-    | inl v => inl v
-    | inr v => inr (SSPF.dep _ _ a v)
-    end
-  end.
-
-Program Definition Depend_Fun : SSPF.t := 
-  @SSPF.mk depfun_Fn _ _ (PNatTrans.mk _ _ depfun_embed _ _) _ _.
-Next Obligation.
-  extensionality s.
-  unfold depfun_map. destruct s. unfold depfun_embed.
-  rewrite PNatTrans.map_nat. simpl. unfold SPUF.map.
-  destruct ((SSPF.emb (B a)) X (x a)); auto.
-Qed.
-Next Obligation.
-  unfold depfun_embed. split; intros.
-  - inversion H. subst.
-    apply (PNatTrans.rel_nat (B a).(SSPF.emb)) in RE.
-    inversion RE. subst.
-    apply (SPUF._u_rel _ (SSPF.dep _ _ a s)).
-    rewrite EQ. auto.
-  - inversion H. subst.
-    destruct s.
-    apply (_depfun_rel x a fx).
-    apply (PNatTrans.rel_nat (B a).(SSPF.emb)).
-    simpl.
-    apply (SPUF._u_rel _ c).
-    destruct ((SSPF.emb (B a)) X (fx a)); inversion EQ. auto.
-Qed.
-Next Obligation.
-  unfold depfun_embed, depfun_map in *.
-  assert (forall a, exists x: (B a) False,
-               m a = PFunctor.map (B a) (fun _ : False => ()) x).
-  { intros.
-    apply (B a).(SSPF.uni). intros.
-    specialize (CONST (SSPF.dep _ _ _ s) x). simpl in CONST.
-    destruct ((SSPF.emb (B a)) _ (m a)).
-    destruct x, u; auto. intro. inversion H.
-  }
-  apply (non_dep_dep_functional_choice choice) in H.
-  destruct H. exists x.
-  extensionality s. apply H.
-Qed.
-Next Obligation.
-  extensionality s. apply SSPF.inj.
-  extensionality sh.
-  unfold depfun_embed in EQ.
-  apply equal_f with (SSPF.dep _ _ _ sh) in EQ.
-  destruct ((SSPF.emb (B s)) X (m s)), ((SSPF.emb (B s)) X (n s));
-  inversion EQ; auto.
-  apply inj_pair2_eq_dec in H0. subst. auto.
-  intros. destruct (excluded_middle_informative (x=y)); auto.
-Qed.
-
-End Dependent_function_SSPF.
-
-Section Dependent_sum_SSPF.
-
-Variable A: Type.
-Variable B: A -> SSPF.t.
-
-Inductive dep_sum X :=
-| dep (a: A) (x': B a X) : dep_sum X.
-
-Definition depsum_map X Y (f: X -> Y) (x: dep_sum X) :=
-  match x with
-  | dep _ a x' =>
-    dep _ a ((B a).(PFunctor.map) f x') end.
-
-Inductive depsum_rel X : X -> dep_sum X -> Prop :=
-| _depsum_rel x a b (RE: (B a).(PFunctor.rel) x b) : depsum_rel x (dep _ a b).
-
-Definition depsum_Fn :=
-  (PFunctor.mk_data dep_sum depsum_map depsum_rel).
-
-Definition depsum_embed X (x: dep_sum X)
-           (s: SSPF.dep_sum B (fun x => sum unit x.(SSPF.Sh))):
-  sum X (sum bool (SSPF.dep_sum B SSPF.Ext)) :=
-  match x with
-  | dep _ a x' =>
-    match s with
-    | SSPF.dep _ _ a' sh =>
-      match (excluded_middle_informative (a = a')) with
-      | left pf =>
-        match sh with
-        | inl _ => inr (inl true)
-        | inr sh' =>
-          match (B a').(SSPF.emb) _ (eq_rect _ (fun y => (B y) X) x' _ pf) sh' with
-          | inl a => inl a
-          | inr b => inr (inr (SSPF.dep _ _ a' b)) end
-        end
-      | right _ => inr (inl false)
-      end
-    end
-  end.
-
-Program Definition Depend_Sum : SSPF.t := 
-  @SSPF.mk depsum_Fn _ _ (PNatTrans.mk _ _ depsum_embed _ _) _ _.
-Next Obligation.
-Proof.
-  extensionality s. unfold depsum_embed, depsum_map, SPUF.map.
-  destruct x; destruct s; destruct c;
-  destruct (excluded_middle_informative (a = a0)); auto.
-  destruct e. simpl.
-  rewrite PNatTrans.map_nat. simpl. unfold SPUF.map.
-  destruct ((SSPF.emb (B a)) X x'); auto.
-Qed.
-Next Obligation.
-  unfold depsum_embed. split; intros.
-  - inversion H. subst.
-    apply (PNatTrans.rel_nat (B a).(SSPF.emb)) in RE.
-    inversion RE. subst.
-    apply (SPUF._u_rel _ (SSPF.dep _ _ a (inr s))).
-    destruct (excluded_middle_informative (a = a)).
-    + rewrite <- eq_rect_eq.
-      destruct ((SSPF.emb (B a)) X b); inversion EQ. auto.
-    + destruct n. auto.
-  - destruct fx.
-    inversion H. subst. clear H.
-    destruct s. destruct c.
-    + destruct (excluded_middle_informative (a = a0)); inversion EQ.
-    + destruct (excluded_middle_informative (a = a0)); subst.
-      rewrite <- eq_rect_eq in EQ.
-      apply (_depsum_rel x a0 _). apply (PNatTrans.rel_nat (B a0).(SSPF.emb)). simpl.
-      apply (SPUF._u_rel _ s).
-      destruct ((SSPF.emb (B a0)) X x'); inversion EQ. auto.
-      inversion EQ.
-Qed.
-Next Obligation.
-  destruct m.
-  unfold depsum_map, depsum_embed in *.
-  assert (forall (s: SSPF.Sh (B a)) (x : unit), (SSPF.emb (B a)) _ x' s <> inl x).
-  { intros.
-    specialize (CONST (SSPF.dep _ _ a (inr s)) x). simpl in CONST.
-    destruct (excluded_middle_informative (a = a)).
-    - assert ((eq_rect a (fun y : A => (B y) unit) x' a e)=x').
-      rewrite <- eq_rect_eq. auto.
-      rewrite H in CONST.
-      destruct ((SSPF.emb (B a)) _ x').
-      destruct u, x. exfalso. auto.
-      intro. inversion H0.
-    - destruct n. auto.
-  }
-  apply SSPF.uni in H.
-  destruct H.
-  exists (dep _ a x). subst. auto.
-Qed.
-Next Obligation.
-  destruct m, n.
-  unfold depsum_embed in EQ.
-  assert (H:= equal_f EQ (SSPF.dep _ _ a (inl tt))).
-  simpl in H.
-  destruct (excluded_middle_informative (a0 = a)). subst.
-  - f_equal. apply SSPF.inj. extensionality s.
-    apply equal_f with (x:= (SSPF.dep _ _ a (inr s))) in EQ.
-    destruct (excluded_middle_informative (a = a)).
-    assert (H1 : (eq_rect a (fun y : A => (B y) X) x' a e) = x').
-    rewrite <- eq_rect_eq. auto.
-    assert (H2 : (eq_rect a (fun y : A => (B y) X) x'0 a e) = x'0).
-    rewrite <- eq_rect_eq. auto.
-    rewrite H1 in EQ. rewrite H2 in EQ.
-    destruct ((SSPF.emb (B a)) X x'), ((SSPF.emb (B a)) X x'0); inversion EQ; auto.
-    apply inj_pair2_eq_dec in H3. subst. auto.
-    intros. destruct (excluded_middle_informative (x=y)); auto.
-    destruct n. auto.
-  - destruct (excluded_middle_informative (a = a)); inversion H.
-    destruct n0. auto.
-Qed.
-
-End Dependent_sum_SSPF.
-
-Section Option_SSPF.
-
-Definition option_rel X (x: X) (o: option X) : Prop :=
-  match o with
-  | Some x' => x = x'
-  | None => False end.
-
-Definition option_Fn :=
-  (PFunctor.mk_data option option_map option_rel).
-
-Definition option_embed X (x: option X) (s: unit) :=
-  match x with
-  | Some x' => inl x'
-  | None => inr tt
-  end.
-
-Program Definition Option_sspf : SSPF.t :=
-   @SSPF.mk option_Fn unit unit 
-           (PNatTrans.mk _ _ option_embed _ _) _ _.
-Next Obligation.
-Proof.
-  destruct x; auto.
-Qed.
-Next Obligation.
-Proof.
-  unfold option_embed. split; intros.
-  - destruct fx; destruct H.
-    apply (SPUF._u_rel _ tt). auto.
-  - inversion H. subst.
-    destruct fx; inversion EQ.
-    simpl. auto.
-Qed.    
-Next Obligation.
-  destruct m; simpl in CONST.
-  - exfalso. apply (CONST tt u). auto.
-  - exists None. auto.
-Qed.
-Next Obligation.
-Proof.
-  apply equal_f with tt in EQ.
-  destruct m, n; inversion EQ; auto.
-Qed.
-
-End Option_SSPF.
