examples.v
@@ -1,36 +1,26 @@
-Require Import FunctionalExtensionality ProofIrrelevance ClassicalDescription.
-Require Import ClassicalChoice ChoiceFacts.
-Require Import Coq.Logic.Eqdep_dec.
 Require Import Program.
 Set Implicit Arguments.
 Set Automatic Coercions Import.
 Require Import ssp combinator fixpoint.
 
-Ltac msimplp := repeat (try simpl; try setoid_rewrite mfix_fn_correct;
-                       try setoid_rewrite mfix_destruct_correct1;
-                       try setoid_rewrite mfix_destruct_correct2).
+Arguments proj1_sig {A P} e.
+Arguments projT1 {A P} x.
+Arguments morder {M y} x OR.
 
-Ltac msimpl := repeat (try simpl; try rewrite mfix_fn_correct;
-                       try rewrite mfix_destruct_correct1;
-                       try rewrite mfix_destruct_correct2).
+Opaque Mfixpoint Mfix_destruct Mfix_mk Mfix_destruct_ord Mfixpoint_fn
+       Mfixpoint_fn_depend destruct_order.
 
-Module Tree.
+Ltac mdestruct x x' := try (rewrite <- (destruct_correct1 x) in *; remember (Mfix_destruct x) as x' eqn : _EQ; clear _EQ; clear x; simpl in x').
 
-Inductive tree : Type :=
-| node : list tree -> tree.
+Ltac minduction x := apply (Mfixpoint_ind' x); intro; intro.
+Ltac minductionr x := apply (Mfixpoint_indr x); intro; intro.
+Ltac msinduction x := apply (Mfixpoint_s_ind x); intro; intro.
 
-Inductive well_founded : tree -> Prop :=
-| wf_leaf : well_founded (node nil)
-| wf_internal hd tl (WHD: well_founded hd) (WTL: well_founded (node tl)) :
-                      well_founded (node (cons hd tl)).
+Ltac minversion H x y := remember x as _a eqn : _EQ1; remember y as _b eqn : _EQ2; 
+apply mfix_mk_inj in H;
+inversion H; repeat rewrite _EQ2 in *; repeat rewrite _EQ1 in *; clear _EQ2; clear _b; clear _EQ1; clear _a.
 
-Theorem tree_well_founded x : well_founded x.
-Proof.
-  induction x.
-Abort.
-
-End Tree.
-
+Ltac minversion2 H x y := remember x as _a eqn : _EQ1; remember y as _b eqn : _EQ2; inversion H; repeat rewrite _EQ2 in *; repeat rewrite _EQ1 in *; clear _EQ2; clear _b; clear _EQ1; clear _a.
 
 Module Tree_SSP.
 
@@ -46,182 +36,194 @@ Inductive well_founded : tree -> Prop :=
 
 Theorem tree_well_founded x : well_founded x.
 Proof.
-  apply Mfixpoint_ind. simpl.
-  induction m; intros.
-  - apply wf_leaf.
-  - dependent destruction IND.
-    apply (wf_internal H (IHm IND)).
+  minductionr x; induction m; simpl in *.
+  - constructor.
+  - apply wf_internal.
+    + apply IND. constructor. constructor.
+    + apply IHm.
+      intros. apply IND.
+      apply inr, X.
 Qed.
 
 End Tree_SSP.
 
 
-Module Option_Nat.
+Section opt_nat.
 
-Definition nat := Mfixpoint (Option_sspf).
+Definition nat := Mfixpoint Option_sspf.
 Definition O := Mfix_mk Option_sspf None.
 Definition S x := Mfix_mk Option_sspf (Some x).
 
-Definition induction_principle n (P: nat -> Prop) (PO : P O) (PS : forall n, P n -> P (S n)) : P n.
-Proof.
-  apply (Mfixpoint_ind n).
-  intros. simpl in IND. unfold option_pmap in IND.
-  destruct m.
-  - apply PS, IND.
-  - apply PO.
-Qed.  
-  
-Inductive le (n: nat) : nat -> Prop := 
-| le_n : le n n
-| le_S : forall m : nat, le n m -> le n (S m).
+Hint Unfold O S.
 
-Definition lt n m := le (S n) m.
+Definition to_nat := Mfixpoint_fn (fun (n: nat) f =>
+  match Mfix_destruct_ord n with
+  | None => 0
+  | Some (morder n' pf) => (f n' pf) + 1 end).
 
-Inductive natural_order (n: nat) : nat -> Prop :=
-| succ : natural_order n (S n). 
-
-Lemma wf : well_founded natural_order.
-Proof.
-  unfold well_founded. intros.
-  apply induction_principle.
-  - constructor.
-    intros.
-    remember O.
-    inversion H.
-    subst.
-    apply (Mfix_mk_inj) in H0.
-    inversion H0.
-  - intros.
-    constructor.
-    intros.
-    remember (S n).
-    inversion H0.
-    inversion Heqm.
-    subst.
-    apply (Mfix_mk_inj) in H1. inversion H1.
-    auto.
-Qed.
-
-Lemma wf2 : well_founded lt.
-Proof.
-  unfold well_founded. intros.
-  apply (induction_principle).
-  - constructor.
-    intros.
-    remember O.    
-    inversion H.
-    + subst.
-      apply (Mfix_mk_inj) in H0.
-      inversion H0.
-    + subst.
-      apply (Mfix_mk_inj) in H1.
-      inversion H1.
-  - intros.
-    constructor.
-    intros.
-    remember (S n).
-    inversion H0.
-    + subst.
-      apply (Mfix_mk_inj) in H1.
-      inversion H1.      
-      subst. auto.
-    + subst.
-      apply (Mfix_mk_inj) in H2.
-      inversion H2.      
-      subst.
-      inversion H.
-      unfold lt at 1 in H3.
-      apply H3, H1.
-Qed.      
-
-Inductive lex : nat * nat -> nat * nat -> Prop := 
-| lex_n : forall n m1 m2, lex (n, m1) (S n, m2)
-| lex_S : forall n m, lex (n, m) (n, S m).
-
-Lemma wf_lex : well_founded lex.
-Proof.
-  unfold well_founded.
-  intros.
-  destruct a.
-  apply (induction_principle n).
-  - constructor.
-    intros.
-    remember O.
-    inversion H;
-    subst.
-    apply (Mfix_mk_inj) in H2.
-    inversion H2.
-    apply (induction_principle m0).
-    + constructor.
-      intros.
-      remember O.
-      inversion H0.
-      subst.
-      apply (Mfix_mk_inj) in H3.
-      inversion H3.
-      subst.
-      apply (Mfix_mk_inj) in H4.
-      inversion H4.
-    + intros.
-      constructor.
-      intros.
-      remember O. remember (S n0).
-      inversion H1.
-      subst.
-      apply (Mfix_mk_inj) in H4.
-      inversion H4.
-      subst.
-      apply (Mfix_mk_inj) in H5.
-      inversion H5.
-      subst.
-      auto.
-    - intros.
-Abort.
-
-Lemma trivalence : forall n m, le n m \/ lt m n.
-Proof.
-  intros.
-Abort.
-
-(* @jeehoonkang: use `Program Definition` *)
-
-Definition fibonacci_gen (_: Option_sspf nat) 
-           (x: Option_sspf (vfx Option_sspf Datatypes.nat)) :=
-  match x with
+Definition fibonacci := Mfixpoint_fn (fun (n: nat) f =>
+  match Mfix_destruct_ord n with
   | None => 1
-  | Some a =>
-    match (mfix_destruct a) with
-    | (None, _) => 1
-    | (Some x', v') =>
-      match (mfix_destruct x') with
-      | (_, v'') => v'' + v' end end end.
+  | Some (morder n' pf1) =>
+    match Mfix_destruct_ord n' with
+    | None => 1
+    | Some (morder n'' pf2) => (f n' pf1) + (f n'' (link_order pf2 pf1)) end end).
 
-Definition fibonacci := mfix_fnd fibonacci_gen.
+Fixpoint to_nat2 (n: Datatypes.nat) : nat :=
+  match n with
+  | Datatypes.O => O
+  | Datatypes.S n' => S (to_nat2 n') end.
 
-Lemma fibonacci_0 : fibonacci O = 1.
+Definition ackermann := Mfixpoint_fn (fun (n: nat) f =>
+  match Mfix_destruct_ord n with
+  | None => (fun m => Mfix_mk Option_sspf (Some m))
+  | Some (morder n' pf1) =>
+    Mfixpoint_fn (fun (m: nat) g =>
+      match Mfix_destruct_ord m with
+      | None => f n' pf1 (Mfix_mk Option_sspf (Some (Mfix_mk Option_sspf None)))
+      | Some (morder m' pf2) => f n' pf1 (g m' pf2) end)
+  end).
+
+(*
+Eval compute in (fibonacci (to_nat2 20)).
+
+Eval compute in (fibonacci (S (S (S (S (S O)))))).
+ = 8
+
+Eval compute in (to_nat (S (S (S (S O))))). 
+ = 4
+
+Eval compute in (to_nat (ackermann (S (S O)) (S (S O)))).
+Eval compute in (ack 2 2).
+
+*)
+
+Lemma fibonacci_c_2 : forall n, fibonacci (S (S n)) = fibonacci (S n) + fibonacci n.
 Proof.
-  unfold fibonacci, mfix_fnd, O.
-  msimpl.
-  auto.
+  intros. unfold fibonacci, S.
+  msimpl. auto.
 Qed.
 
-Lemma fibonacci_1 : fibonacci (S O) = 1.
+Lemma ackermann_c_1 : forall n, ackermann O n = S n.
 Proof.
-  unfold fibonacci, mfix_fnd, O, S.
-  msimpl.
-  auto.
+  intros. unfold ackermann, O, S.
+  msimpl. auto.
 Qed.
 
-Lemma fibonacci_SS x : fibonacci (S (S x)) = fibonacci x + fibonacci (S x).
+Lemma ackermann_c_2 : forall m, ackermann (S m) O = ackermann m (S O).
 Proof.
-  unfold fibonacci, mfix_fnd, O, S.
-  msimpl.
-  destruct (@mfix_destruct (Prod Option_sspf (Const Datatypes.nat))
-        (@mfix_fn Option_sspf (vfx Option_sspf Datatypes.nat)
-           (fun (mfx : option (Mfixpoint Option_sspf))
-              (mvfx : option (vfx Option_sspf Datatypes.nat)) =>
-            Mfix_mk (Prod Option_sspf (Const Datatypes.nat))
-              (@pair (option (vfx Option_sspf Datatypes.nat)) Datatypes.nat mvfx
-                 (fibonacci_gen mfx mvfx))) x)).
-  auto.
+  intros. unfold ackermann, O, S.
+  msimpl. auto. 
 Qed.
+
+Lemma ackermann_c_3 : forall m n, ackermann (S m) (S n) = ackermann m (ackermann (S m) n).
+Proof.
+  intros. unfold ackermann, O, S.
+  msimpl. auto. 
+Qed.
+
+(* TODO induction and inversion tactic*)
+
+Definition pred (n: nat) :=
+  match Mfix_destruct n with
+  | None => Mfix_mk Option_sspf None
+  | Some x => x end.
+
+Definition evenb := Mfixpoint_fn (fun (n:nat) f =>
+  match Mfix_destruct_ord n with
+  | None => true
+  | Some (morder n' pf1) =>
+    match Mfix_destruct_ord n' with
+    | None => false
+    | Some (morder n'' pf2) => f n'' (link_order pf2 pf1) end end).
+
+Definition oddb (n:nat) : bool := negb (evenb n).
+
+Definition plus := Mfixpoint_fn (fun (n : nat) f =>
+(fun (m : nat) =>
+  match Mfix_destruct_ord n with
+  | None => m
+  | Some (morder n' pf) => Mfix_mk Option_sspf (Some (f n' pf m)) end)).
+
+Definition mult := Mfixpoint_fn (fun (n: nat) f =>
+(fun (m : nat) =>
+  match Mfix_destruct_ord n with
+  | None => Mfix_mk Option_sspf None
+  | Some (morder n' pf) => plus m (f n' pf m)
+  end)).
+
+Definition minus := Mfixpoint_fn (fun (n: nat) f =>
+(fun (m: nat) => 
+  match Mfix_destruct_ord n with
+  | None => Mfix_mk Option_sspf None
+  | Some (morder n' pf) =>
+    match Mfix_destruct m with
+    | None => n
+    | Some m' => f n' pf m' end end)).
+
+Definition exp (base: nat) := Mfixpoint_fn (fun (power : nat) f =>
+  match Mfix_destruct_ord power with
+  | None => Mfix_mk Option_sspf (Some (Mfix_mk Option_sspf None))
+  | Some (morder p pf) => mult base (f p pf) end).
+
+Notation "x + y" := (plus x y)
+                       (at level 50, left associativity)
+                       : nat_scope.
+Notation "x - y" := (minus x y)
+                       (at level 50, left associativity)
+                       : nat_scope.
+Notation "x * y" := (mult x y)
+                       (at level 40, left associativity)
+                       : nat_scope.
+
+Theorem plus_n_O : forall n:nat, n = n + (Mfix_mk Option_sspf None).
+Proof.
+  intro n. minductionr n. destruct m; unfold plus in *; simpl in IND.
+  - specialize (IND m (eq_refl m)).
+    rewrite IND at 1. msimpl. auto.
+  - msimpl. auto.
+Qed.
+
+Theorem plus_n_Sm : forall n m : nat,
+  Mfix_mk Option_sspf (Some (n + m)) = n + (Mfix_mk Option_sspf (Some m)).
+Proof.
+  intro. minductionr n. destruct m; unfold plus in *.
+  - msimpl. intro.
+    specialize (IND m (eq_refl m) m0). msimpl_in IND.
+    rewrite IND. auto.
+  - msimpl. auto.
+Qed.
+
+Theorem plus_comm : forall n m : nat,
+  n + m = m + n.
+Proof.
+  intro. minductionr n; destruct m.
+  - intro. unfold plus. msimpl. fold plus.
+    rewrite IND.
+    apply plus_n_Sm.
+    constructor.
+  - intro. unfold plus. msimpl.
+    apply plus_n_O.
+Qed.
+
+Inductive lt : nat -> nat -> Prop :=
+| lt_base n : lt n (S n)
+| lt_stem n m : lt n m -> lt n (S m).
+
+Definition bbb (n: nat) :=
+  match Mfix_destruct n with
+  | None => 1
+  | Some n' => 1 end.
+
+Lemma bbb1 n : bbb n = 1.
+Proof.
+  mdestruct n a. destruct a; unfold bbb; msimpl; auto.
+Qed.
+
+Lemma sss n : S (S n) = S O -> False.
+Proof.
+  intros. apply mfix_mk_inj in H.
+  inversion H.
+Qed.
+
+End opt_nat.
