fixpoint.v
@@ -1,12 +1,10 @@
-Require Import FunctionalExtensionality ProofIrrelevance ClassicalDescription.
-Require Import ClassicalChoice ChoiceFacts.
-Require Import Coq.Logic.Eqdep_dec.
 Require Import Program.
 Set Implicit Arguments.
 Set Automatic Coercions Import.
 Require Import ssp combinator.
 
 Arguments proj1_sig {A P} e.
+Arguments projT1 {A P} x.
 
 Section SSPF_Fixpoint.
 
@@ -15,46 +13,131 @@ Variable M: SSPF.t.
 Inductive Mfixpoint_ : Type :=
 | Mfix_mk_ : SPUF.U M.(SSPF.Sh) M.(SSPF.Ext) Mfixpoint_ -> Mfixpoint_.
 
-(* @jeehoonkang: why `unique` in OnHD? *)
-Inductive PMfixpoint : Mfixpoint_ -> Prop :=
-| PMfix_mk m (OnHD: ex (unique (SSPF.on_image M m))) (OnTL: SPUF.pmap PMfixpoint m)
-  : PMfixpoint (Mfix_mk_ m).
-Hint Constructors PMfixpoint.
+Inductive PMfixpoint : Mfixpoint_ -> Type :=
+| PMfix_mk (m: M Mfixpoint_)
+           (OnTL: forall x, SPUF.u_mem (M.(SSPF.emb) _ m) x -> PMfixpoint x)
+  : PMfixpoint (Mfix_mk_ (M.(SSPF.emb) _ m)).
 
-Definition Mfixpoint := sig PMfixpoint.
+Definition Mfixpoint : Type := sigT PMfixpoint.
 
-Definition Mfix_mk (m : M Mfixpoint) : Mfixpoint :=
-  exist _ (Mfix_mk_ (SPUF.map _ _ proj1_sig (M.(SSPF.emb) _ m)))
-        (PMfix_mk (SSPF.sig_on_image _ _ m) (SSPF.sig_all _ _)).
+Definition Mfix_mk_prop (m : M Mfixpoint)
+  : PMfixpoint (Mfix_mk_ (M.(SSPF.emb) _ (M.(PFunctor.map) projT1 m))).
+Proof.
+  constructor. intros.
+  inversion X. subst.
+  rewrite SSPF.map_nat in EQ. unfold SPUF.map in EQ.
+  destruct ((SSPF.emb M) Mfixpoint m); inversion EQ.
+  destruct m0. simpl. auto.
+Defined.
 
-Inductive order_Mfix_ : Mfixpoint_ -> Mfixpoint_ -> Prop:=
-| _order_Mfix_ x u : SPUF.u_rel x u -> order_Mfix_ x (Mfix_mk_ u).
+Definition Mfix_mk (m: M Mfixpoint) : Mfixpoint := existT _ _ (Mfix_mk_prop m).
+
+Definition Mfix_destruct' (x: Mfixpoint_) (p: PMfixpoint x) : M Mfixpoint_ :=
+  match p with
+  | PMfix_mk m OnTL => m end.
+
+Definition Mfix_destruct_all (x: Mfixpoint_) (p: PMfixpoint x)
+           : forall y, M.(PFunctor.mem) (Mfix_destruct' p) y -> Mfixpoint.
+  intros. econstructor.
+  destruct p.
+  apply SSPF.mem_nat1 in X. simpl in X.
+  apply OnTL in X. apply X.
+Defined.
+
+Definition Mfix_destruct (x: Mfixpoint) : M Mfixpoint :=
+  match x with
+  | existT _ _ p => M.(PFunctor.uni) _ (Mfix_destruct_all p) end.
+
+Inductive order_Mfix_' : Mfixpoint_ -> Mfixpoint_ -> Type :=
+| _order_Mfix_' x u : SPUF.u_mem u x -> order_Mfix_' x (Mfix_mk_ u).
+
+Inductive order_Mfix_ : Mfixpoint_ -> Mfixpoint_ -> Prop :=
+| _order_Mfix_ a b : order_Mfix_' a b -> order_Mfix_ a b.
 
 Lemma wf_order_Mfix_ : well_founded order_Mfix_.
 Proof.
   unfold well_founded. fix 1. intro. destruct a.
   constructor. intros.
-  inversion H. inversion H2.
+  inversion H. inversion X. inversion X0.
   destruct (u s).
-  - specialize (wf_order_Mfix_ m). inversion EQ.
-    rewrite H6 in wf_order_Mfix_.
+  - specialize (wf_order_Mfix_ m). inversion EQ. subst.
     apply wf_order_Mfix_.
   - inversion EQ.
+Defined.
+
+Lemma Mfix__ind x (P: Mfixpoint_ -> Prop)
+    (STEP: forall m (IND: forall y, order_Mfix_ y m -> P y), P m):
+  P x.
+Proof.
+  apply (Fix wf_order_Mfix_ _ STEP).
+Defined.
+
+(* test *)
+
+Lemma PMfixpoint_unique x : forall (p1 : PMfixpoint x) (p2 : PMfixpoint x), p1 = p2.
+Proof.
+  apply (Mfix__ind x). clear x.
+  dependent destruction p1.
+  dependent destruction p2.
+  apply SSPF.inj in x0. subst.
+  assert (OnTL = OnTL0).
+  extensionality s. extensionality r.
+  specialize (IND s (_order_Mfix_ (_order_Mfix_' r))).
+  apply IND.
+  subst. auto.
+Qed.
+
+Lemma mfix_mk'_unique : forall (x1 x2: Mfixpoint_) p1 p2,
+    existT PMfixpoint x1 p1 = existT PMfixpoint x2 p2 -> x1 = x2.
+Proof.
+  intros.
+  inversion H. auto.
+Qed.
+
+Lemma mfix_mk'_unique2 : forall (x1 x2: Mfixpoint_) p1 p2,
+    x1 = x2 -> existT PMfixpoint x1 p1 = existT PMfixpoint x2 p2.
+Proof.
+  intros.
+  subst.
+  replace p1 with p2. auto.
+  apply PMfixpoint_unique.
+Qed.
+
+Lemma mfix_mk_inj m1 m2 (EQ: Mfix_mk m1 = Mfix_mk m2) : m1 = m2.
+Proof.
+  apply mfix_mk'_unique in EQ. inversion EQ.
+  apply SSPF.inj. extensionality s.
+  apply equal_f with s in H0.
+  repeat rewrite SSPF.map_nat in H0. unfold SPUF.map in H0.
+  destruct (SSPF.emb M _ m1), (SSPF.emb M _ m2); inversion H0.
+  - destruct m, m0. simpl in H1. subst.
+    repeat f_equal. apply PMfixpoint_unique.
+  - auto.
+Qed.
+
+Lemma destruct_correct1 x : Mfix_mk (Mfix_destruct x) = x.
+Proof.
+  destruct x. destruct p. unfold Mfix_mk. simpl.
+  apply mfix_mk'_unique2.
+  f_equal. f_equal.
+  apply M.(PFunctor.uni_correct). auto.
+Qed.
+
+Lemma destruct_correct2 m : Mfix_destruct (Mfix_mk m) = m.
+Proof.
+  apply mfix_mk_inj.
+  apply destruct_correct1.
 Qed.
 
 Inductive order_Mfix : Mfixpoint -> Mfixpoint -> Prop:=
-| _order_Mfix x m : M.(PFunctor.rel) x m -> order_Mfix x (Mfix_mk m).
+| _order_Mfix m1 p1 m2 p2 : order_Mfix_ m1 m2 ->
+                            order_Mfix (existT _ m1 p1) (existT _ m2 p2).
 
 Lemma order_Mfix_preserve m1 m2 (ORD: order_Mfix m1 m2) :
-  order_Mfix_ (proj1_sig m1) (proj1_sig m2).
+  order_Mfix_ (projT1 m1) (projT1 m2).
 Proof.
-  inversion ORD.
-  apply (PNatTrans.rel_nat M.(SSPF.emb)) in H. simpl in H.
-  inversion H. subst.
-  unfold Mfix_mk. simpl.
-  constructor.
-  apply SPUF.u_rel_map. auto.
-Qed.
+  inversion ORD. auto.
+Defined.
 
 Lemma acc_preserve X Y (f: X -> Y) (Rx : X -> X -> Prop) (Ry : Y -> Y -> Prop)
       (H: forall x1 x2 (RE: Rx x1 x2), Ry (f x1) (f x2)) (WF: well_founded Ry )y :
@@ -68,7 +151,7 @@ Proof.
   apply H0.
   apply H3.
   auto.
-Qed.
+Defined.
 
 Lemma sub_wellorder X Y (f: X -> Y) (Rx : X -> X -> Prop) (Ry : Y -> Y -> Prop)
       (H: forall x1 x2 (RE: Rx x1 x2), Ry (f x1) (f x2)) (WF: well_founded Ry) 
@@ -76,24 +159,20 @@ Lemma sub_wellorder X Y (f: X -> Y) (Rx : X -> X -> Prop) (Ry : Y -> Y -> Prop)
 Proof.
   unfold well_founded. intros. apply (@acc_preserve _ _ f Rx _ H WF (f a)).
   auto.
-Qed.
+Defined.
 
 Lemma wf_order_Mfix : well_founded order_Mfix.
 Proof.
-  apply (sub_wellorder proj1_sig _ order_Mfix_preserve wf_order_Mfix_).
-Qed.
-
-Inductive Mfix_with_order y : Type :=
-| morder x (OR: order_Mfix x y) : Mfix_with_order y.
+  apply (sub_wellorder projT1 _ order_Mfix_preserve wf_order_Mfix_).
+Defined.
 
 Lemma Mfixpoint_ind' x (P: Mfixpoint -> Prop)
     (STEP: forall m (IND: forall y, order_Mfix y m -> P y), P m):
   P x.
 Proof.
   apply (Fix wf_order_Mfix _ STEP).
-Qed.
+Defined.
 
-(* @jeehoonkang: use standard library one.. *)
 Inductive s_order_Mfix : Mfixpoint -> Mfixpoint -> Prop :=
 | base_order x y (RE: order_Mfix x y) : s_order_Mfix x y
 | step_order x y z (Rxy: s_order_Mfix x y) (Ryz: order_Mfix y z) : s_order_Mfix x z.
@@ -107,7 +186,7 @@ Proof.
   - apply IND, RE.
   - specialize (IND y Ryz).
     destruct IND. eauto.
-Qed.
+Defined.
 
 Lemma link_order x y z (Rxy: s_order_Mfix x y) (Ryz: s_order_Mfix y z) :
   s_order_Mfix x z.
@@ -119,58 +198,14 @@ Proof.
   - apply (step_order Rxy RE).
   - specialize (IND _ Ryz0 Rxy Ryz).
     apply (step_order IND Ryz0).
-Qed.
+Defined.
 
-Inductive Mfix_with_s_order y : Type :=
-| msorder x (OR: s_order_Mfix x y) : Mfix_with_s_order y.
+Inductive Mfix_with_order y : Type :=
+| morder x (OR: s_order_Mfix x y) : Mfix_with_order y.
 
-Definition Mfix_get y (x: Mfix_with_order y) : Mfixpoint :=
-match x with
-| @morder _ x' _ => x' end.
-
-Definition Mfix_s_get y (x: Mfix_with_s_order y) : Mfixpoint :=
-match x with
-| @msorder _ x' _ => x' end.
-
-Definition Mfixpoint_destruct (x: Mfixpoint) : M Mfixpoint.
-Admitted.
-
-Lemma destruct_correct1 (x: Mfixpoint) : Mfix_mk (Mfixpoint_destruct x) = x.
-Admitted.
-
-Lemma destruct_correct2 (m: M Mfixpoint) : Mfixpoint_destruct (Mfix_mk m) = m.
-Admitted.
-
-Definition ordered_destruct (x: Mfixpoint) : M (Mfix_with_order x).
-Admitted.
-
-Definition s_ordered_destruct (x: Mfixpoint) : M (Mfix_with_s_order x).
-Admitted.
-
-Lemma Mfix_with_order_correct x : M.(PFunctor.map) (@Mfix_get x) (ordered_destruct x) = Mfixpoint_destruct x.
-Admitted.
-
-Lemma Mfix_with_s_order_correct x : M.(PFunctor.map) (@Mfix_s_get x) (s_ordered_destruct x) = Mfixpoint_destruct x.
-Admitted.
-
-Lemma Mfixpoint_ind x (P: Mfixpoint -> Prop)
-    (STEP: forall m (IND: forall y, M.(PFunctor.rel) y m -> P y), P (Mfix_mk m)):
-  P x.
-Proof.
-  assert (H : forall m (IND: forall y, order_Mfix y m -> P y), P m). intros.
-  rewrite <- (destruct_correct1 m) in *. apply STEP.
-  intros. apply IND. constructor. apply H.
-  apply (Mfixpoint_ind' x _ H).
-Qed.
-
-(* @jeehoonkang: don't use `P` for types *)
-Definition Mfixpoint_fn_depend (P: Mfixpoint -> Type)
-    (FIX: forall m (FN: forall y, order_Mfix y m -> P y), P m) : forall x, P x :=
-  Fix wf_order_Mfix _ FIX.
-
-Definition Mfixpoint_fn T
-    (FIX: forall m (FN: forall y, order_Mfix y m -> T), T) x : T :=
-  Fix wf_order_Mfix _ FIX x.
+Definition Mfix_v_get y (x: Mfix_with_order y) : Mfixpoint :=
+  match x with
+  | @morder _ x' _ => x' end.
 
 Lemma Mfixpoint_s_ind x (P: Mfixpoint -> Prop)
     (STEP: forall m (IND: forall y, s_order_Mfix y m -> P y), P m):
@@ -179,36 +214,278 @@ Proof.
   apply (Fix wf_s_order_Mfix _ STEP).
 Qed.
 
-Definition Mfixpoint_s_fn_depend (P: Mfixpoint -> Type)
+Definition Mfixpoint_fn_depend (P: Mfixpoint -> Type)
     (FIX: forall m (FN: forall y, s_order_Mfix y m -> P y), P m) : forall x, P x :=
   Fix wf_s_order_Mfix _ FIX.
 
-Definition Mfixpoint_s_fn T
+Definition Mfixpoint_fn T
     (FIX: forall m (FN: forall y, s_order_Mfix y m -> T), T) x : T :=
   Fix wf_s_order_Mfix _ FIX x.
 
-Lemma Mfixpoint_s_fn_correct T
+Lemma Fix_F_eq A (R : A -> A -> Prop) (P : A -> Type) (F : forall x: A, (forall y:A, R y x -> P y) -> P x) :
+  forall (x : A) (r: Acc R x),
+  @F x (fun (y : A) (p : R y x) => @Fix_F A R P F y (@Acc_inv A R x r y p)) = Fix_F P F r.
+Proof.
+  intros. destruct r. simpl. auto.
+Qed.
+
+Lemma Fix_correct A (R : A -> A -> Prop) (P : A -> Type) (F : forall x: A, (forall y:A, R y x -> P y) -> P x) (W : well_founded R) :
+  forall x, F x (fun y _ => (Fix W P F y)) = Fix W P F x.
+Proof.
+  intros. unfold Fix.
+  rewrite <- (Fix_F_eq _ _ (W x)).
+  f_equal. extensionality s1. extensionality s2.
+  f_equal. apply proof_irrelevance.
+Qed.
+
+Lemma Mfixpoint_fn_correct T
       (FIX: forall m (FN: forall y, s_order_Mfix y m -> T), T) x :
-  Mfixpoint_s_fn FIX x = FIX x (fun y _ => Mfixpoint_s_fn FIX y).
-Admitted.
-
-Lemma Mfix_mk_inj (m1 m2: M Mfixpoint) (EQ: Mfix_mk m1 = Mfix_mk m2): m1 = m2.
+  Mfixpoint_fn FIX (Mfix_mk x) = FIX (Mfix_mk x) (fun y _ => Mfixpoint_fn FIX y).
 Proof.
-  unfold Mfix_mk in EQ. dependent destruction EQ.
-  apply SPUF.map_injective in x.
-  - apply M.(SSPF.inj) in x. auto.
-  - intros. destruct x1, x2. simpl in EQ; subst.
-    rewrite (proof_irrelevance _ p p0). auto.
+  unfold Mfixpoint_fn. 
+  rewrite <- Fix_correct. auto.
 Qed.
 
-Lemma order_correct a b : order_Mfix a (Mfix_mk b) <-> M.(PFunctor.rel) a b.
+Lemma Mfixpoint_fn_correct2 T
+      (FIX: forall m (FN: forall y, s_order_Mfix y m -> T), T) x :
+  Mfixpoint_fn FIX x = FIX x (fun y _ => Mfixpoint_fn FIX y).
 Proof.
-  split; intros.
-  - remember (Mfix_mk b). inversion H.
-    subst. apply Mfix_mk_inj in H2. subst. apply H0.
-  - constructor. apply H.
+  unfold Mfixpoint_fn. 
+  rewrite <- Fix_correct. auto.
 Qed.
 
-(* TODO fn_correct *)
+Lemma Mfixpoint_fn_d_correct (P: Mfixpoint -> Type)
+    (FIX: forall m (FN: forall y, s_order_Mfix y m -> P y), P m) x :
+  Mfixpoint_fn_depend P FIX (Mfix_mk x) 
+  = FIX (Mfix_mk x) (fun y _ => Mfixpoint_fn_depend P FIX y).
+Proof.
+  unfold Mfixpoint_fn_depend. 
+  rewrite <- Fix_correct. auto.
+Qed.
+
+Lemma Mfixpoint_fn_d_correct2 (P: Mfixpoint -> Type)
+    (FIX: forall m (FN: forall y, s_order_Mfix y m -> P y), P m) x :
+  Mfixpoint_fn_depend P FIX x = FIX x (fun y _ => Mfixpoint_fn_depend P FIX y).
+Proof.
+  unfold Mfixpoint_fn_depend. 
+  rewrite <- Fix_correct. auto.
+Qed.
+
+Definition Mfix_destruct_all_ord (x: Mfixpoint_) (p: PMfixpoint x)
+           : forall y, M.(PFunctor.mem) (Mfix_destruct' p) y -> Mfix_with_order (existT _ _ p).
+  intros.
+  destruct p.
+  set X. apply SSPF.mem_nat1 in m0.
+  set m0.
+  apply OnTL in u.
+  apply _order_Mfix_' in m0.
+  apply _order_Mfix_ in m0.
+  set (_order_Mfix u (PMfix_mk m OnTL) m0). 
+  apply base_order in o.
+  apply morder in o.
+  apply o.
+Defined.
+
+Definition Mfix_destruct_ord (x: Mfixpoint) : M (Mfix_with_order x) :=
+match x with
+| existT _ _ p => M.(PFunctor.uni) _ (Mfix_destruct_all_ord p) end.
+
+Definition order_correct1 m x : PFunctor.mem M m x -> order_Mfix x (Mfix_mk m).
+Proof.
+  intros. destruct x.
+  constructor. constructor. constructor.
+  apply SSPF.mem_nat1 in X.
+  inversion X. subst.
+  apply (SPUF._u_mem _ s).
+  rewrite SSPF.map_nat. unfold SPUF.map. simpl in *.
+  destruct (SSPF.emb M Mfixpoint m); inversion EQ. auto.
+Defined.
+
+Definition order_correct2 m x (ORD: order_Mfix x (Mfix_mk m))
+  : inhabited (PFunctor.mem M m x).
+Proof.
+  inversion ORD. inversion H1. inversion X. inversion X0. subst.
+  constructor. apply SSPF.mem_nat2.
+  apply (SPUF._u_mem _ s).
+  rewrite SSPF.map_nat in EQ. unfold SPUF.map in EQ.
+  destruct (SSPF.emb M Mfixpoint m); inversion EQ.
+  destruct m0. simpl in H0. subst.
+  f_equal. f_equal. apply PMfixpoint_unique.
+Qed.
+
+Lemma Mfixpoint_indr x (P: Mfixpoint -> Prop)
+    (STEP: forall m (IND: forall y, M.(PFunctor.mem) m y -> P y), P (Mfix_mk m)):
+  P x.
+Proof.
+  assert (H : forall m (IND: forall y, order_Mfix y m -> P y), P m). intros.
+  rewrite <- (destruct_correct1 m) in *. apply STEP.
+  intros. apply IND.
+  apply (order_correct1 _ _ X).
+  apply (Mfixpoint_ind' x _ H).
+Qed.
+
+Definition destruct_order m : forall x, M.(PFunctor.mem) m x -> s_order_Mfix x (Mfix_mk m).
+  intros. destruct x. unfold Mfix_mk.
+  repeat constructor.
+  apply SSPF.mem_nat1 in X.
+  inversion X. subst.
+  apply (SPUF._u_mem _ s).
+  rewrite SSPF.map_nat. unfold SPUF.map.
+  destruct (SSPF.emb M Mfixpoint m); inversion EQ.
+  auto.
+Defined.
+
+Lemma destruct_ord_correct m 
+  : Mfix_destruct_ord (Mfix_mk m) 
+    = M.(PFunctor.uni) m (fun x r => morder (destruct_order m x r)).
+Proof.
+  apply SSPF.map_injective with (f := (fun x => projT1 (Mfix_v_get x))).
+  - intros. destruct x1, x2. destruct x, x0.
+    simpl in EQ. subst.
+    assert (EQ := PMfixpoint_unique p p0). subst.
+    f_equal. apply proof_irrelevance.
+  - simpl. rewrite PFunctor.uni_correct.
+    replace (PFunctor.map M (fun x  => projT1 (Mfix_v_get x))
+    (PFunctor.uni M m (fun x r => morder (destruct_order m x r)))) with
+        (PFunctor.map M projT1 (PFunctor.map M (@Mfix_v_get _)
+                                             (PFunctor.uni M m (fun x r =>
+                                                morder (destruct_order m x r))))).
+    f_equal. rewrite PFunctor.uni_correct. auto.
+    { intros. auto. }
+    apply M.(PFunctor.map_comp).
+    { intros. auto. }
+Qed.
+
+Definition prim_rec T (f: M T -> T) := Mfixpoint_fn (fun (m: Mfixpoint) g =>
+  let g' (m': Mfix_with_order m) : T :=
+    match m' with
+    | @morder _ m'' r => g m'' r end in
+  f (M.(PFunctor.map) g' (Mfix_destruct_ord m))).
+
+Lemma prim_rec_correct T (f: M T -> T) m :
+  prim_rec f (Mfix_mk m) = f (M.(PFunctor.map) (prim_rec f) m).
+Proof.
+  unfold prim_rec. rewrite Mfixpoint_fn_correct.
+  f_equal. rewrite destruct_ord_correct.
+  remember (Mfixpoint_fn
+           (fun (m0 : Mfixpoint) (g : forall y : Mfixpoint, s_order_Mfix y m0 -> T)
+            =>
+            f
+              (PFunctor.map M
+                 (fun m'0 : Mfix_with_order m0 =>
+                  match m'0 with
+                  | @morder _ m''0 r0 => g m''0 r0
+                  end) (Mfix_destruct_ord m0)))) as g.
+  replace (fun m' : Mfix_with_order (Mfix_mk m) =>
+     match m' with
+     | @morder _ m'' _ => g m''
+     end) with (fun m' => g (@Mfix_v_get (Mfix_mk m) m')).
+  rewrite <- M.(PFunctor.map_comp).
+  f_equal. apply PFunctor.uni_correct.
+  intros. auto.
+  { extensionality s.
+    destruct s eqn : EQ.
+    auto.
+  }
+Qed.
 
 End SSPF_Fixpoint.
+
+
+Section Deep_Recursion.
+
+Variable M : SSPF.t.
+
+Definition vfx T := Mfixpoint (Prod M (Const T)).
+
+Definition mfix_fnd T (tfix: M (vfx T) -> T) (x: Mfixpoint M) :=
+  let tfix' (mvfx : M (vfx T)) : vfx T :=
+      Mfix_mk (Prod M (Const T)) (mvfx, tfix mvfx) in
+  match Mfix_destruct (prim_rec tfix' x) with
+  | (_, t) => t end.
+
+End Deep_Recursion.
+
+Opaque Mfixpoint Mfix_destruct Mfix_mk Mfix_destruct_ord Mfixpoint_fn
+       Mfixpoint_fn_depend prim_rec destruct_order.
+
+Ltac msimpl := repeat (repeat rewrite Mfixpoint_fn_correct;
+                       repeat rewrite Mfixpoint_fn_d_correct;
+                       repeat rewrite prim_rec_correct;
+                       repeat rewrite destruct_ord_correct;
+                       repeat rewrite Mfixpoint_fn_d_correct;
+                       repeat rewrite destruct_correct1;
+                       repeat rewrite destruct_correct2;
+                       simpl).
+
+Ltac msimpl_in H := repeat (repeat rewrite Mfixpoint_fn_correct in H;
+                       repeat rewrite Mfixpoint_fn_d_correct in H;
+                       repeat rewrite prim_rec_correct in H;
+                       repeat rewrite destruct_ord_correct in H;
+                       repeat rewrite Mfixpoint_fn_d_correct in H;
+                       repeat rewrite destruct_correct1 in H;
+                       repeat rewrite destruct_correct2 in H;
+                       simpl in H).
+
+Section Mlist.
+
+Variable M : SSPF.t.
+Variable X : Type.
+
+Definition F := Coprod (Const unit) (Prod (Const (M X)) M).
+
+Definition Mlist := Mfixpoint F.
+
+Definition Mnil := Mfix_mk F (inl tt).
+Definition Mcons (hd : M X) (tl : M Mlist) := Mfix_mk F (inr (hd, tl)).
+
+Lemma Mcons_inj h1 t1 h2 t2
+    (EQ: Mcons h1 t1 = Mcons h2 t2):
+  h1 = h2 /\ t1 = t2.
+Proof.
+  assert (H := @mfix_mk_inj F _ _ EQ).
+  inversion H. eauto.
+Qed.
+
+Lemma Mcons_inj2 hd tl (EQ: Mcons hd tl = Mnil):
+  False.
+Proof.
+  assert (H := @mfix_mk_inj F _ _ EQ).
+  inversion H.
+Qed.
+
+Lemma Mlist_ind l (P: Mlist -> Prop)
+    (BASE: P Mnil)
+    (STEP: forall hd tl 
+             (IND: forall x, M.(PFunctor.mem) tl x -> P x), 
+           P (Mcons hd tl)):
+  P l.
+Proof.
+  apply (@Mfixpoint_indr F l P).
+  intros. destruct m.
+  - destruct f. exact BASE.
+  - destruct f. apply STEP.
+    intros. apply IND. apply (inr X0).
+Qed.
+
+Definition mfix T (tnil: T) (tcons: M X -> M T -> T) (l: Mlist) : T :=
+  @prim_rec F T (fun m => 
+                   match m with
+                   | inl tt => tnil
+                   | inr (mx, mt) => tcons mx mt end) l.
+
+Lemma mfix_correct_cons T (tnil: T) (tcons: M X -> M T -> T) hd tl : 
+  mfix tnil tcons (Mcons hd tl) = tcons hd (PFunctor.map M (mfix tnil tcons) tl).
+Proof.
+  unfold mfix, Mcons.
+  msimpl. auto.
+Qed.
+
+Lemma mfix_correct_nil T (tnil: T) (tcons: M X -> M T -> T) :
+  mfix tnil tcons Mnil = tnil.
+Proof.
+  unfold mfix, Mnil.
+  msimpl. auto.
+Qed.
+
+End Mlist.
